lib/lib/Meta/Opaque.lean
@@ -1,11 +1,39 @@
 
 import Lean.Elab.Declaration
+import Lean.Elab.Command
+import Lean.Elab.BuiltinCommand
 
 import Lib.Meta
+import Lib.Meta.Dump
+import Lib.Meta.TransportFacts
 
-def Option.elim {α β} (x : β) (f : α → β) : Option α → β
-| Option.none => x
-| Option.some x => f x
+namespace Option
+
+def elim {α β} (x : β) (f : α → β) : Option α → β
+| none => x
+| some x => f x
+
+end Option
+
+namespace Std.AssocList
+
+variable [DecidableEq α]
+
+def eraseAll (x : α) : AssocList α β → AssocList α β
+| nil => nil
+| cons k v xs =>
+  let xs' := eraseAll x xs
+  if x = k then xs'
+  else cons k v xs'
+
+end Std.AssocList
+
+namespace Lean.Meta
+
+def applyc (g : MVarId) (n : Name) : MetaM (List MVarId) := do
+apply g (← mkConstWithFreshMVarLevels n)
+
+end Lean.Meta
 
 structure Locked {α : Sort u} (x : α) where
   val : α
@@ -13,6 +41,115 @@ structure Locked {α : Sort u} (x : α) where
 
 namespace Lean
 namespace Parser
+namespace OpaqueExt
+
+open Lean.Elab.Tactic
+open Lean
+
+structure OpaqueDef where
+  declName : Name
+  intlName : Name
+  eqvProof : Name
+  lockedConst : Name
+  unfoldEqn : Option Name := none
+  eqns : Array Name := #[]
+  deriving Inhabited
+
+-- #check Lean.Meta.simp
+-- #check Lean.Meta.SimpTheorems
+
+structure OpaqueDefIdx where
+  intlToDecl : NameMap OpaqueDef := {}
+  decls : NameMap OpaqueDef := {}
+  simpLemmas : Lean.Meta.SimpTheorems := {}
+  newLemmas : List Name := []
+  -- newLemmas : Std.AssocList Name Name := Std.AssocList.nil
+  deriving Inhabited
+
+namespace OpaqueDefIdx
+
+def insert (o : OpaqueDefIdx) (decl : OpaqueDef) : OpaqueDefIdx where
+  intlToDecl := o.intlToDecl.insert decl.intlName decl
+  decls := o.intlToDecl.insert decl.declName decl
+  simpLemmas := o.simpLemmas
+  newLemmas := decl.eqvProof :: o.newLemmas
+  -- newLemmas := Std.AssocList.cons decl.intlName decl.eqvProof o.newLemmas
+  -- simpLemmas := (← o.simpLemmas.addConst (inv := true) decl.eqvProof) }
+
+def erase (o : OpaqueDefIdx) (decl : Name) : OpaqueDefIdx := Id.run do
+let some d := o.decls.find? decl
+  | return o
+return {
+  decls := o.decls.erase decl
+  intlToDecl := o.intlToDecl.erase d.intlName
+  simpLemmas := o.simpLemmas.eraseCore d.eqvProof
+  newLemmas := o.newLemmas.erase d.eqvProof
+  }
+
+end OpaqueDefIdx
+
+abbrev OpaqueExtension :=
+SimpleScopedEnvExtension OpaqueDef OpaqueDefIdx
+
+
+def mkOpaqueExt (extName : Name) : IO OpaqueExtension :=
+  registerSimpleScopedEnvExtension {
+    name     := extName
+    initial  := {}
+    addEntry := fun d decl => d.insert decl
+    -- addEntry := fun d e => d.insert e
+  }
+
+def getOpaqueExtension (ext : OpaqueExtension) : MetaM OpaqueDefIdx := do
+return ext.getState (← getEnv)
+-- return ext.getState env
+
+def getEqnsForOpaqueDef (ext : OpaqueExtension) (n : Name) : MetaM (Option (Array Name)) := do
+return (← getOpaqueExtension ext)
+  |>.decls
+  |>.find? n
+  |>.map (·.eqns)
+
+def getUnfoldEqnsForOpaqueDef (ext : OpaqueExtension) (n : Name) : MetaM (Option Name) := do
+return (← getOpaqueExtension ext)
+  |>.decls
+  |>.find? n
+  |>.bind (·.unfoldEqn)
+
+def registerOpaqueAttr (attrName : Name) (attrDescr : String) (extName : Name := attrName.appendAfter "Ext") : IO OpaqueExtension := do
+  let ext ← mkOpaqueExt extName
+  Lean.Meta.registerGetEqnsFn <| getEqnsForOpaqueDef ext
+  Lean.Meta.registerGetUnfoldEqnFn <| getUnfoldEqnsForOpaqueDef ext
+  -- mkOpaqueAttr attrName attrDescr ext
+  return ext
+
+end OpaqueExt
+
+initialize opaqueExtension : OpaqueExt.OpaqueExtension ← OpaqueExt.registerOpaqueAttr `opaque "opaque definitions"
+
+def getOpaqueExtension :=
+OpaqueExt.getOpaqueExtension opaqueExtension
+
+def setOpaqueExtension (idx : OpaqueExt.OpaqueDefIdx) : MetaM Unit :=
+modifyEnv λ env => opaqueExtension.modifyState env λ _ => idx
+
+def registerOpaqueDef (decl : OpaqueExt.OpaqueDef) : MetaM Unit := do
+-- let env ← getEnv
+modifyEnv (opaqueExtension.addEntry . decl)
+
+
+def getSimpLemmas : MetaM Meta.SimpTheorems := do
+-- let simps
+let ext ← getOpaqueExtension
+let mut simpLemmas := ext.simpLemmas
+for eqn in ext.newLemmas do
+  simpLemmas ← simpLemmas.addConst (inv := true) eqn
+setOpaqueExtension <| { ext with
+  newLemmas := []
+  simpLemmas := simpLemmas }
+return simpLemmas
+
+
 namespace Command
 
 open Elab Elab.Command
@@ -23,6 +160,7 @@ syntax (name := opaqueDef)
 
 -- opaque struct, instance, inductive
 
+initialize registerTraceClass `opaque
 initialize registerTraceClass `opaque.decls
 
 def proveNewEqn (t₀ : Expr) (eqnN name name' defN : Name) : MetaM Name := do
@@ -49,57 +187,354 @@ let c' ← mkConstWithLevelParams name'
 let t := t.replace λ e => if e == c' then some c else none
 proveNewEqn t eqn name name' eqThm
 
-def constantWrapper (name name' : Name) : MetaM Unit := do
-  let ls := (← getConstInfo name').levelParams
-  let e ← mkConstWithLevelParams name'
+def constantWrapper (declName intlName : Name) : MetaM Unit := do
+  let ls := (← getConstInfo intlName).levelParams
+  let ls' := ls.map mkLevelParam
+  let e ← mkConstWithLevelParams intlName
 
   let t ← inferType e
   let t' ← mkAppOptM ``Locked #[none, e]
   let eqPr ← mkAppOptM ``rfl #[none, e]
   let locked ← mkAppOptM ``Locked.mk #[none, e, e, eqPr]
-  let name'' ← addConst ls (name ++ `_locked) t' locked
-  trace[opaque.decls]"constant {name''} : {t'} := {locked}"
+  -- trace[opaque.decl]"foo {lockedName}"
+  let lockedName ← addConst ls (declName ++ `_locked) t' locked
+  trace[opaque.decls]"constant {lockedName} : {t'} := {locked}"
 
-  let locked_e ← mkConstWithLevelParams name''
+  let locked_e ← mkConstWithLevelParams lockedName
   let e' ← mkAppOptM ``Locked.val #[none, none, locked_e]
-  trace[opaque.decls]"def {name} : {t} := {e'}"
-  discard <| addDef ls name t e'
+  trace[opaque.decls]"def {declName} : {t} := {e'}"
+  discard <| addDef ls declName t e'
 
-  let e_def ← mkConstWithLevelParams name
+  let e_def ← mkConstWithLevelParams declName
   let pr ← mkAppOptM ``Locked.val_eq #[none, none, locked_e]
   let eqStmt ← mkAppOptM ``Eq #[none, e_def, e]
-  let eqThmName := name ++ `_unlock
+  let eqThmName := declName ++ `_unlock
   trace[opaque.decls]"theorem {eqThmName} : {eqStmt}"
   let eqThm ← addThm ls eqThmName eqStmt pr
-  let eqns := (← getEqnsFor? name') |>.getD #[]
-  let uEqns : Array Name := (← getUnfoldEqnFor? name')
-    |>.elim #[] <| #[].push
-  let newEqns ← eqns.mapM (rewriteEqn . name name' eqThm)
-  let newUEqns ← uEqns.mapM (rewriteEqn . name name' eqThm)
+  let eqns := (← getEqnsFor? intlName) |>.getD #[]
+  -- let uEqns : Array DeclName := (← getUnfoldEqnFor? intlName)
+  let uEqns : Option Name ← getUnfoldEqnFor? intlName
+    -- |>.elim #[] <| #[].push
+  let newEqns  ← eqns.mapM (rewriteEqn . declName intlName eqThm)
+  let newUEqns ← uEqns.mapM (rewriteEqn . declName intlName eqThm)
+  let t ← mkAppOptM ``Transport.EqvTerm
+    #[none, none, none, mkConst declName ls', mkConst intlName ls']
+  let eqC := mkConst eqThm ls'
+  -- let eqSymm ←  mkAppOptM ``Eq.symm #[none,none,none,mkConst eqThm ls']
+  let eqvInst ← mkAppOptM ``Transport.EqvTerm.ofEq #[none, none, none, eqC]
+  let inst ← addDef ls (declName ++ `instEqvTerm) t eqvInst
+  addInstance inst AttributeKind.«global» 0
+  print_vars![withType eqvInst]
+
+  let opDef : OpaqueExt.OpaqueDef :=
+    { declName := declName,
+      intlName := intlName,
+      eqvProof := eqThm,
+      lockedConst := lockedName,
+      eqns := newEqns,
+      unfoldEqn := newUEqns }
+  registerOpaqueDef opDef
   pure ()
+
+#check @Transport.EqvTerm.ofEq
 
 def replaceName (n n' : Name) (s : Syntax) := Id.run <|
 s.replaceM λ s =>
   if s.isIdent && s.getId == n then
-    mkIdentFrom s n'
+    return mkIdentFrom s n'
   else none
+-- #check @mkDeclName
+
+section Name
+open Name
+
+def mkImplName : Name → Name
+| str p s _ => p ++ mkSimple s ++ `_impl ++ mkSimple s
+| n => n
+
+#eval mkImplName `a.b.c
+
+end Name
 
 @[commandElab opaqueDef]
 def elabOpaqueDef : CommandElab := λ stx => do
   let mods := stx[0]
   let kw := stx[1]
   let «def» := stx[2]
-  let name  := «def»[1][0].getId
-  let name' := name ++ `_def
-  let id    := «def»[1].setArg 0 <| Lean.mkIdent name'
+  let declName  := «def»[1][0].getId
+  let ns ← getCurrNamespace
+  let insideName := mkImplName declName
+  trace[opaque.decls]"impl name: {insideName}"
+  let id    := «def»[1].setArg 0 <| Lean.mkIdent insideName
   let «def» := «def».setArg 1 id
-  let «def» := replaceName name `_def «def»
+  -- let «def» := replaceName declName `_def «def»
   let stx   := mkNode ``Lean.Parser.Command.declaration #[mods, «def»]
   let ppStx ← liftCoreM <| Lean.PrettyPrinter.ppCommand stx
   trace[opaque.decls]"{ppStx}"
+  -- let n ← runTermElabM (some declName) λ _ => do
+    -- mkDeclDeclName (← getCurrDeclNamespace) {} declName
+  -- trace[opaque.decls]"declName: {declName}"
+  trace[opaque.decls]"declNamespace: {ns}"
   Lean.Elab.Command.elabDeclaration stx
-  liftTermElabM none <| constantWrapper name name'
+  let declName   := ns ++ declName
+  let insideName := ns ++ insideName
+  liftTermElabM none <| constantWrapper declName insideName
 
 end Command
+namespace Transport
+
+open OpaqueExt
+
+-- #fullname liftTermElabM
+-- #fullname AttrM
+-- #pred Lean.AttrM
+-- #pred Lean.CoreM
+-- #path Lean.Elab.Term.TermElabM Lean.CoreM
+-- #succ Lean.Elab.Term.TermElabM
+-- #check Lean.AttrM
+
+-- #path Syntax Format
+
+-- #check Lean.Syntax.formatStx
+-- #check Lean.Syntax.prettyPrint
+-- #fullname liftMetaM
+-- #check Lean.Meta.liftMetaM
+
+-- #fullname rewriteExpr
+-- #find prefix replace
+-- #check Lean.Expr.replace
+-- elab_rules : command
+-- | `($d:declaration) => println!"my elab"
+-- let env ← getEnv
+
+def transportType (e : Expr) : MetaM Expr := do
+let idx ← getOpaqueExtension
+return e.replace λ
+  | (Expr.const n ls _) =>
+    match idx.intlToDecl.find? n with
+    | some d => mkConst d.declName ls
+    | none => none
+  | _ => none
+
+open Lean.Meta
+open Transport
+open Lean.Elab
+open Lean.Parser.Tactic
+open Lean.Elab.Tactic
+open Lean.Elab.Term
+-- #check LockedType
+-- #check @Transport.mkLockedType
+-- #fullname TacticM
+-- #check TacticM
+-- #find prefix repeat
+-- #fullname first
+-- #find prefix first
+
+partial def repeat (tac : TacticM Unit) : TacticM Unit := do
+let b ← tryTactic tac
+if b then repeat tac
+else return ()
+
+def liftMetaTactic1' (tac : MVarId → MetaM (α × MVarId)) : TacticM α := do
+let (x, g) ← liftMetaMAtMain (tac .)
+replaceMainGoal [g]
+return x
+
+def proveTransport (g : Expr) : TermElabM Expr := do
+let g ← mkFreshExprMVar g
+discard <| Tactic.run g.mvarId! do
+  repeat <| withMainContext do
+
+    let g ← getMainTarget
+    -- print_vars! [g]
+    discard (liftMetaTactic1' intro1) <|>
+    liftMetaTactic1 (do Meta.assumption .; return none) <|>
+    liftMetaTactic (Meta.applyc . ``Transport.EqvTypes_arrow) <|>
+    liftMetaTactic (Meta.applyc . ``Transport.EqvTypes_forall) <|>
+    liftMetaTactic (Meta.applyc . ``Transport.EqvTerm_app) <|>
+    liftMetaTactic (Meta.applyc . ``Transport.EqvTypes_of_EqvTerm) <|>
+    liftMetaTactic (Meta.applyc . ``inferInstance)
+  let gs ← getUnsolvedGoals
+  for g in gs do
+    print_vars![asGoal g]
+    -- setGoals [g]
+    -- liftMetaTactic (Meta.applyc . ``Transport.EqvTypes_arrow)
+  done
+-- intro1
+-- guard gs.isEmpty <|> throwError "cannot generate complete proof"
+-- print_vars! [withType g]
+instantiateMVars g
+
+    -- solve
+    -- | repeat
+    --     first
+    --     | intros _
+    --     | assumption
+    --     | apply EqvTypes_arrow
+    --     | apply EqvTypes_forall
+    --     | apply EqvTerm_app
+    --     | apply EqvTypes_of_EqvTerm
+    --     | exact inferInstance )
+
+-- def listMVars (e : Expr) : List MVarId :=
+-- Expr.replace
+
+-- #find prefix isArrow
+-- #check Lean.Expr.isArrow
+def transportDecl (declName intlName : Name) : MetaM Unit := do
+        let c  ← mkConstWithLevelParams intlName
+        let t  ← inferType c
+        let t' ← transportType t
+        print_vars![t', t]
+        -- let v  ← mkFreshExprMVar none
+        let e ← mkAppOptM ``Transport.mkLockedType #[t',none,c]
+        let argT := (← inferType e).bindingDomain!
+        print_vars![argT]
+        -- let e := e.bindingDomain!
+        let transPr ← proveTransport argT |>.run'
+        let pr := mkApp e transPr
+        -- print_vars![t, withType pr]
+        let ls  := (← getConstInfo intlName) |>.levelParams
+        let ls' := ls.map mkLevelParam
+        print_vars![t']
+        -- print_vars![t, t', withType e, argT, withType pr]
+        println!"*** ABC ***"
+        let prT ← inferType pr
+        let pr' ← instantiateMVars pr
+        let mvars := (← getMVarsNoDelayed pr).map asGoal
+        print_vars![prT, prT.hasMVar, pr.hasMVar, pr'.hasMVar, mvars]
+        let lockedDecl ← addConst ls (declName ++ `_locked)
+            (← inferType pr) pr
+        println!"*** ABC ***"
+        -- TODO: decl, eqv thm, EqvTerm instance, add in extension
+        let lockedC := mkConst lockedDecl ls'
+        let e ← mkAppOptM ``LockedType.val
+          #[none, none, none, lockedC]
+        discard <| addDef ls declName t' e
+        let declC := mkConst declName ls'
+        let intlC := mkConst intlName ls'
+        let e ← mkAppOptM ``LockedType.val_eqv #[none, none, none, lockedC]
+        let heq ← mkAppOptM ``HEq #[none, declC, none, intlC]
+        print_vars![heq, withType e]
+        let unlock ← addThm ls (declName ++ `_unlock) heq e
+
+        println!"*** B ***"
+        print_vars![withType declC, withType intlC]
+        let instT ← mkAppOptM ``Transport.EqvTerm
+          #[none,none,transPr,declC,intlC]
+        print_vars![instT]
+        println!"*** C ***"
+        let heqPr := mkConst unlock ls'
+        println!"*** A ***"
+        print_vars![asConst ``Transport.EqvTerm.ofHEq, typeOf transPr, typeOf heqPr]
+        let instPr ← mkAppOptM ``Transport.EqvTerm.ofHEq
+          #[none,none,transPr,none,none,heqPr]
+        println!"*** C ***"
+        let inst ← addThm ls (declName ++ `instEqvTerm) instT instPr
+        addInstance inst AttributeKind.«global» 0
+        println!"*** D ***"
+
+        let opDef : OpaqueExt.OpaqueDef :=
+          { declName := declName,
+            intlName := intlName,
+            eqvProof := unlock,
+            lockedConst := lockedDecl,
+            eqns := #[],
+            unfoldEqn := none }
+        registerOpaqueDef opDef
+
+
+        print_vars![asConst lockedDecl, asConst declName,
+                    asConst unlock, asConst inst]
+
+-- #check @Transport.EqvTerm
+-- #check @HEq.symm
+#check @Transport.EqvTerm.ofHEq
+
+
+open Lean.Elab.Command
+
+private def removeImpl : Name → Name
+| Name.str p _ _ => p
+| n => n
+
+def elabAndTransport (n : Name) (d : Syntax) : CommandElabM Unit := do
+let ns ← getCurrNamespace
+let «def» := d.getArgs[1]
+let kind := «def».getKind
+let rawName := «def»[1][0].getId
+let intlName := ns ++ rawName
+let declName := removeImpl ns ++ rawName
+elabDeclaration d
+if kind == `Lean.Parser.Command.def then
+  print_vars![ns, intlName, declName]
+-- let opName := stx.getArg 1 |>.getId
+-- println!"id: {opName}"
+  liftCoreM <| transportDecl declName intlName |>.run'
+
+println!"hello {n}"
+
+-- #find prefix ela
+-- #check Lean.Elab.Command.elabEnd
+
+def myElabEnd (n : Name) : CommandElabM Unit := do
+-- λ s => println!"my end elab"
+elabEnd (← `(end $(Lean.mkIdent <| n ++ `_impl):ident))
+
+macro "opaque " "namespace " id:ident : command => do
+  let implName := Lean.mkIdent <| id.getId ++ `_impl
+  let idStr := Lean.Syntax.mkStrLit id.getId.toString
+  -- let defName := Lean.mkIdent <| id.getId ++ `_def
+  let command := Lean.mkIdent `command
+  let idLit := Lean.Syntax.mkNameLit <| toString id
+  let implNLit := Lean.Syntax.mkNameLit "_impl"
+  `(
+
+    namespace $implName:ident
+    -- local notation $idStr => $defName
+    local elab_rules : $command
+    | `($$d:declaration) => elabAndTransport $idLit:nameLit d
+
+    -- not working
+    local elab_rules : $command
+    | `(end $$id') => Lean.Parser.Transport.myElabEnd id'.getId
+    -- | s@`(end $$id') => elabEnd <| id' ++ $implNLit:nameLit
+
+    )
+
+-- #fullname command
+
+-- #pred AttrM
+-- #check AttrM
+def mkOpaqueAttr (attrName : Name) (attrDescr : String) (ext : OpaqueExtension) : IO Unit :=
+  registerBuiltinAttribute {
+    name  := attrName
+    descr := attrDescr
+    add   := fun implName stx attrKind => do
+        -- let t ← Lean.Meta.MetaM.run'  `(attr| transport id)
+        if stx.getNumArgs != 2 then
+          throwError "bad syntax"
+        let opName := stx.getArg 1 |>.getId
+        println!"id: {opName}"
+        transportDecl opName implName |>.run'
+        -- Command.constantWrapper opDecl implName  |>.run'
+        -- | _ =>
+          -- let kinds := stx.getKind :: (stx.getArgs.map (·.getKind)).toList
+          -- throwError "bad syntax for `transport`: {stx.prettyPrint}\n{kinds}"
+    erase := fun declName => do
+      let s := ext.getState (← getEnv)
+      let s := s.erase declName
+      modifyEnv fun env => ext.modifyState env fun _ => s
+  }
+
+syntax (name := transport) "transport" ident : attr
+
+initialize
+  mkOpaqueAttr `transport "descr" opaqueExtension
+
+
+end Transport
+
+
 end Parser
 end Lean
