lib/lib/Meta/deBruijn.lean
@@ -1,25 +1,190 @@
 
 import Lib.Data.Nat
+import Lib.Data.Ordering
+import Lib.Data.List.Basic
+import Lib.Meta.DeclGraph
 import Lib.Meta.Opaque
+import Lib.Order.Basic
 
 namespace Fin
 open Nat
+@[simp]
 protected def succ {n} : Fin n → Fin (succ n)
 | ⟨i,h⟩ => ⟨i.succ, Nat.succ_lt_succ h⟩
 
+def last : Fin (succ n) := ⟨n, Nat.lt_succ_self _⟩
+
+@[simp]
 def widen {n} : Fin n → Fin (succ n)
 | ⟨i,h⟩ => ⟨i, Nat.lt_succ_of_le <| Nat.le_of_lt h⟩
 
+def split {m n} : Fin (m + n) → Fin m ⊕ Fin n
+| ⟨i, h⟩ =>
+  if h' : i < m
+  then Sum.inl ⟨i, h'⟩
+  else
+    have : i - m < n :=
+      Nat.sub_lt_of_lt_add
+        (Nat.le_of_not_gt h') (Nat.add_comm n m ▸ h)
+    Sum.inr ⟨i - m, this⟩
+
+def cast (h : m = n) : Fin m → Fin n
+| ⟨i, h'⟩ => ⟨i, h ▸ h'⟩
+
+def cutl : (i : Fin (m + n)) → i.val < m → Fin m
+| ⟨i, h⟩, h' => ⟨i, h'⟩
+
+def cutr : (i : Fin (m + n)) → ¬ i.val < m → Fin n
+| ⟨i, h⟩, h' =>
+  have : i - m < n :=
+    Nat.sub_lt_of_lt_add
+      (Nat.le_of_not_gt h') (Nat.add_comm n m ▸ h)
+  ⟨i - m, this⟩
+
+def cutl' : (i : Fin (n + m)) → i.val < m → Fin m
+| ⟨i, h⟩, h' => ⟨i, h'⟩
+
+def cutr' : (i : Fin (n + m)) → ¬ i.val < m → Fin n
+| ⟨i, h⟩, h' =>
+  have : i - m < n :=
+    Nat.sub_lt_of_lt_add
+      (Nat.le_of_not_gt h') (Nat.add_comm n m ▸ h)
+  ⟨i - m, this⟩
+
+@[simp]
+theorem val_last :
+  (@Fin.last n).val = n := rfl
+
+@[simp]
+theorem val_cast (h : m = n) (i : Fin m) :
+  (i.cast h).val = i := rfl
+
+@[simp]
+theorem val_cutl (i : Fin (m + n)) h :
+  (i.cutl h).val = i.val := rfl
+
+@[simp]
+theorem val_cutr (i : Fin (m + n)) h :
+  (i.cutr h).val = i.val - m := rfl
+
+@[simp]
+theorem val_cutl' (i : Fin (m + n)) h :
+  (i.cutl' h).val = i.val := rfl
+
+@[simp]
+theorem val_cutr' (i : Fin (m + n)) h :
+  (i.cutr' h).val = i.val - n := rfl
+
+theorem val_inj {x y : Fin n} (h : x.val = y.val) : x = y :=
+by cases x; cases y; cases h; refl
+
 end Fin
+
+namespace List
+
+theorem get_eq_of_eq_0 {xs : List α} (i : Fin _)
+        (h : i.val = 0) :
+  (x :: xs).get i = x := by
+cases i; cases h
+simp [List.get]
+
+end List
+
+namespace Bool
+
+-- @[simp]
+-- theorem and_eq_true : (x && y) = true ↔ x = true ∧ y = true := by
+-- cases x <;> cases y <;> simp
+
+@[simp]
+theorem decide_eq_true [H : Decidable p] :
+  decide p = true ↔ p := by
+cases H <;> simp [decide] <;> assumption
+
+end Bool
+
+
+namespace Lean
+namespace Name
+
+-- @[simp]
+-- theorem beq_anonymous :
+--   (anonymous == anonymous) = true := rfl
+
+-- @[simp]
+-- theorem beq_num :
+--   (num p n h == num p' n' h') = true ↔
+--   (p == p') = true ∧ n = n' :=
+-- by simp [BEq.beq, Name.beq] <;> auto
+
+-- @[simp]
+-- theorem beq_str :
+--   (str p n h == str p' n' h') = true ↔
+--   (p == p') = true ∧ n = n' ∧ h = h' :=
+-- by simp [BEq.beq, Name.beq] <;> auto
+
+-- theorem beq_iff_eq {n n' : Name} :
+--   n == n' ↔ n = n' := by
+-- induction n generalizing n'
+-- <;> cases n'
+-- <;> next =>
+--   constructor <;> simp [*] <;> intro h
+--   <;> try (cases h) <;> try auto
+
+-- #exit
+instance : DecidableEq Name
+| n, n' =>
+  withPtrEqDecEq n n' λ () =>
+    match n, n' with
+    | anonymous, anonymous => isTrue rfl
+    | str p n h, str p' n' h' =>
+      have hh := (inferInstanceAs (Decidable (h = h')))
+      have hn := (inferInstanceAs (Decidable (n = n')))
+      have hp := instDecidableEqName p p'
+      have h := @instDecidableAnd _ _ hh (@instDecidableAnd _ _ hn hp)
+      @Decidable.congr _ _ h <| by
+        constructor <;> intro h
+        next =>
+          repeat
+            first
+            | rfl
+            | apply congr
+          all_goals auto
+        next => cases h; auto
+    | num p n h, num p' n' h' =>
+      have hh := (inferInstanceAs (Decidable (h = h')))
+      have hn := (inferInstanceAs (Decidable (n = n')))
+      have hp := instDecidableEqName p p'
+      have h := @instDecidableAnd _ _ hh (@instDecidableAnd _ _ hn hp)
+      @Decidable.congr _ _ h <| by
+        constructor <;> intro h
+        next =>
+          repeat
+            first
+            | rfl
+            | apply congr
+          all_goals auto
+        next => cases h; auto
+    | num _ _ _, str _ _ _ => isFalse λ h => by cases h
+    | num _ _ _, anonymous => isFalse λ h => by cases h
+    | str _ _ _, num _ _ _ => isFalse λ h => by cases h
+    | str _ _ _, anonymous => isFalse λ h => by cases h
+    | anonymous, num _ _ _ => isFalse λ h => by cases h
+    | anonymous, str _ _ _ => isFalse λ h => by cases h
+
+end Name
+end Lean
 
 
 inductive Typ : Type
 | nat | bool | arrow (t₀ t₁ : Typ)
 
 open Nat
+open Lean (Name)
+
 inductive Term' : Nat → Type
 | bvar {n} : Fin n → Term' n
-| fvar {n} : String → Term' n
+| fvar {n} : Name → Term' n
 | plus {n} (t₀ t₁ : Term' n) : Term' n
 | ite {n} (c t₀ t₁ : Term' n) : Term' n
 | app {n} (t₀ t₁ : Term' n) : Term' n
@@ -36,17 +201,242 @@ def bump (k : Nat) : Term' n → Term' (succ n)
 | app t₀ t₁ => app (bump k t₀) (bump k t₁)
 | lam T t => lam T (bump k.succ t)
 
-def subst (v : String) (e : Term' n) : Term' n → Term' n
+def subst (v : Name) (e : Term' n) : Term' n → Term' n
 | bvar i => bvar i
 | fvar v' =>
-  if v = v' then e else fvar v'
+  if v == v' then e else fvar v'
 | plus t₀ t₁ => plus (subst v e t₀) (subst v e t₁)
 | Term'.ite c t₀ t₁ =>
   ite (subst v e c) (subst v e t₀) (subst v e t₁)
 | app t₀ t₁ => app (subst v e t₀) (subst v e t₁)
 | lam T t' => lam T (subst v (bump 0 e) t')
 
-inductive Occurs : {n : Nat} → String → Term' n → Prop
+-- #print _sizeOf_inst
+-- #pred sizeOf
+
+-- inductive Subterm : ((n : Nat) × Term' n) → ((n : Nat) × Term' n) → Prop
+-- | plus₀ {n} {t₀ t₁ : Term' n} : Subterm ⟨n, t₀⟩ ⟨n, plus t₀ t₁⟩
+-- | plus₁ {n} {t₀ t₁ : Term' n} : Subterm ⟨n, t₁⟩ ⟨n, plus t₀ t₁⟩
+-- | app₀ {n} {t₀ t₁ : Term' n} : Subterm ⟨n, t₀⟩ ⟨n, app t₀ t₁⟩
+-- | app₁ {n} {t₀ t₁ : Term' n} : Subterm ⟨n, t₁⟩ ⟨n, app t₀ t₁⟩
+-- | itec {n} {c t₀ t₁ : Term' n} : Subterm ⟨n, c⟩ ⟨n, Term'.ite c t₀ t₁⟩
+-- | ite₀ {n} {c t₀ t₁ : Term' n} : Subterm ⟨n, t₀⟩ ⟨n, Term'.ite c t₀ t₁⟩
+-- | ite₁ {n} {c t₀ t₁ : Term' n} : Subterm ⟨n, t₁⟩ ⟨n, Term'.ite c t₀ t₁⟩
+-- | lam {n} {T} {t : Term' _} : Subterm ⟨_, t⟩ ⟨n, lam T t⟩
+
+-- @[simp]
+def height : Term' n → Nat
+| bvar _ => 0
+| fvar _ => 0
+-- | plus t₀ t₁ => 1 + height t₀ + height t₁
+| plus t₀ t₁ => height t₀ + height t₁ + 1
+| app t₀ t₁ => height t₀ + height t₁ + 1
+| Term'.ite c t₀ t₁ => height c + height t₀ + height t₁ + 1
+| lam T t => height t + 1
+
+-- namespace sizeOf
+
+-- variable {c t₀ t₁ : Term' n}
+-- variable (i : Fin 0)
+-- -- #eval sizeOf (@bvar 1 ⟨0, Nat.zero_lt_one⟩)
+-- #reduce sizeOf (bvar i)
+
+-- theorem _eq_1  : sizeOf (bvar i) = 1 :=
+-- show n.succ = _ from _
+
+-- end sizeOf
+
+
+-- set_option pp.explicit true in
+-- #check @sizeOf (Term' _) _
+-- #succ Term'
+-- #exit
+
+-- inductive A := | a
+
+-- def termWf : WellFoundedRelation ((n : Nat) × Term' n) where
+--   rel := Subterm
+--   wf := by
+--     constructor; intro a; cases a
+--     next n t =>
+--     induction t <;> constructor
+--     <;> intro a <;> cases a <;> intro h
+--     <;> cases h <;> assumption
+
+-- #check measure
+-- #check Nat.le_add_left
+attribute [scoped auto] Nat.le_add_left Nat.le_add_right Nat.succ_le_succ
+
+-- open Ordering in
+-- def inst {n} (k : Fin (succ n)) (e : Term' n) : Term' (succ n) → Term' n
+-- | bvar i =>
+--   match compare i.val k.val, rfl : (o : Ordering) → compare i.val k = o → _ with
+--   | eq, h => e
+--   | lt, h =>
+--     -- have h₀ : i.val < k.val := sorry
+--     have h₀ : i.val < k.val := by
+--       simp at h; assumption
+--     have h₁ : k.val ≤ n := Nat.le_of_succ_le_succ k.isLt
+--     bvar ⟨i.val, Nat.lt_of_lt_of_le h₀ h₁⟩
+--   | gt, h =>
+--     -- have : 1 ≤ i.val := sorry
+--     have : 1 ≤ i.val := by
+--       simp at h; trans _ </> assumption
+--       auto
+--     have : i.val - 1 < n := Nat.sub_lt_of_lt_add this i.isLt
+--     bvar ⟨i.val - 1,  this⟩
+-- | fvar v => fvar v
+-- | plus t₀ t₁ =>
+--        have : height t₀ < height (plus t₀ t₁) :=
+--          by simp [height];
+--             apply Nat.succ_le_succ
+--             apply Nat.le_add_right
+--          -- by simp [height]; auto
+--        have : height t₁ < height (plus t₀ t₁) :=
+--          by simp [height];
+--             apply Nat.succ_le_succ
+--             apply Nat.le_add_left
+--             -- apply Nat.le_add_of_le_r
+--          --    -- apply Nat.le_add_right
+--          -- by simp [height]; auto
+--        plus (inst k e t₀) (inst k e t₁)
+-- | Term'.ite c t₀ t₁ =>
+--        have : height c  < height (ite c t₀ t₁) :=
+--          by simp [height];
+--             apply Nat.succ_le_succ
+--             apply Nat.le_add_of_le_l
+--          --    -- apply Nat.le_add_right
+--             apply Nat.le_add_right
+--        have : height t₀ < height (ite c t₀ t₁) :=
+--          by simp [height];
+--             apply Nat.succ_le_succ
+--             apply Nat.le_add_of_le_l
+--          --    -- apply Nat.le_add_right
+--             apply Nat.le_add_left
+--          --    -- auto with 10
+--        have : height t₁ < height (ite c t₀ t₁) :=
+--          by simp [height];
+--             apply Nat.succ_le_succ
+--             -- apply Nat.le_add_of_le_l
+--             apply Nat.le_add_left
+--        ite (inst k e c) (inst k e t₀) (inst k e t₁)
+-- | app t₀ t₁ =>
+--        have : height t₀ < height (app t₀ t₁) :=
+--          by simp [height]
+--             apply Nat.succ_le_succ
+--             apply Nat.le_add_right
+--          -- by simp [height]; auto
+--        have : height t₁ < height (app t₀ t₁) :=
+--          by simp [height]
+--             apply Nat.succ_le_succ
+--             apply Nat.le_add_left
+--          --    -- auto with 17
+--        app (inst k e t₀) (inst k e t₁)
+-- | lam T t' =>
+--   -- have : height t' < height (lam T t') :=
+--          -- by simp [height]
+--             -- apply Nat.succ_le_succ
+--             -- apply Nat.le_add_left
+--             -- auto with 17
+--   lam T (inst k.succ (bump 0 e) t')
+-- -- termination_by' inst n k e t => Sigma.mk n t
+-- termination_by inst t => height t
+-- -- decreasing_by simp [InvImage]; try auto
+
+open POrdering DecidableTotalOrder in
+def inst' {n} (k : Fin n) (e : Term' m) (hn : n = m.succ) :
+  Term' n → Term' m
+| bvar i =>
+  -- have ⟨a, h⟩ : { a // compare i.val k.val = a } :=
+    -- ⟨ _,  rfl ⟩
+  match pcompare i.val k.val with
+  | isEQ h => e
+  | isLT h =>
+    have h₀ : i.val < k.val := by
+      simp at h; assumption
+    have h₁ : k.val ≤ m := Nat.le_of_succ_le_succ <| hn ▸ k.isLt
+    bvar ⟨i.val, Nat.lt_of_lt_of_le h₀ h₁⟩
+  | isGT h =>
+    have : 1 ≤ i.val := by
+      simp at h
+      trans k.val.succ <;> auto
+    have : i.val - 1 < m := Nat.sub_lt_of_lt_add this <| hn ▸ i.isLt
+    bvar ⟨i.val - 1,  this⟩
+| fvar v => fvar v
+| plus t₀ t₁ =>
+       -- have : height t₀ < height (plus t₀ t₁) :=
+       --   by simp [height];
+       --      apply Nat.succ_le_succ
+       --      apply Nat.le_add_right
+       --   -- by simp [height]; auto
+       -- have : height t₁ < height (plus t₀ t₁) :=
+       --   by simp [height];
+       --      apply Nat.succ_le_succ
+       --      apply Nat.le_add_left
+       --      -- apply Nat.le_add_of_le_r
+       --   --    -- apply Nat.le_add_right
+       --   -- by simp [height]; auto
+       plus (inst' k e hn t₀) (inst' k e hn t₁)
+| Term'.ite c t₀ t₁ =>
+       -- have : height c  < height (ite c t₀ t₁) :=
+       --   by simp [height];
+       --      apply Nat.succ_le_succ
+       --      apply Nat.le_add_of_le_l
+       --   --    -- apply Nat.le_add_right
+       --      apply Nat.le_add_right
+       -- have : height t₀ < height (ite c t₀ t₁) :=
+       --   by simp [height];
+       --      apply Nat.succ_le_succ
+       --      apply Nat.le_add_of_le_l
+       --   --    -- apply Nat.le_add_right
+       --      apply Nat.le_add_left
+       --   --    -- auto with 10
+       -- have : height t₁ < height (ite c t₀ t₁) :=
+       --   by simp [height];
+       --      apply Nat.succ_le_succ
+       --      -- apply Nat.le_add_of_le_l
+       --      apply Nat.le_add_left
+       ite (inst' k e hn c) (inst' k e hn t₀) (inst' k e hn t₁)
+| app t₀ t₁ =>
+       -- have : height t₀ < height (app t₀ t₁) :=
+       --   by simp [height]
+       --      apply Nat.succ_le_succ
+       --      apply Nat.le_add_right
+       --   -- by simp [height]; auto
+       -- have : height t₁ < height (app t₀ t₁) :=
+       --   by simp [height]
+       --      apply Nat.succ_le_succ
+       --      apply Nat.le_add_left
+       --   --    -- auto with 17
+       app (inst' k e hn t₀) (inst' k e hn t₁)
+| lam T t' =>
+  -- have : height t' < height (lam T t') :=
+         -- by simp [height]
+            -- apply Nat.succ_le_succ
+            -- apply Nat.le_add_left
+            -- auto with 17
+  lam T (inst' k.succ (bump 0 e) (congrArg _ hn) t')
+-- termination_by' inst n k e t => Sigma.mk n t
+-- termination_by inst t => height t
+-- decreasing_by simp [InvImage]; try auto
+
+def inst {n} (k : Fin (succ n)) (e : Term' n) : Term' (succ n) → Term' n :=
+inst' k e rfl
+
+def abstr {n} (v : Name) (k : Fin (succ n)) : Term' n → Term' (succ n)
+| bvar i =>
+  if k.val ≤ i.val then bvar i.succ
+  else bvar i.widen
+| fvar v' =>
+  if v = v' then bvar k
+  else fvar v'
+| plus t₀ t₁ => plus (abstr v k t₀) (abstr v k t₁)
+| app t₀ t₁ => app (abstr v k t₀) (abstr v k t₁)
+| ite c t₀ t₁ => ite (abstr v k c) (abstr v k t₀) (abstr v k t₁)
+| lam T t => lam T (abstr v k.succ t)
+
+@[auto]
+inductive Occurs : {n : Nat} → Name → Term' n → Prop
 | fvar : Occurs (n := n) v (fvar v)
 | plus₀ {t₀ t₁ : Term' n} : Occurs v t₀ → Occurs v (plus t₀ t₁)
 | plus₁ {t₀ t₁ : Term' n} : Occurs v t₁ → Occurs v (plus t₀ t₁)
@@ -57,11 +447,80 @@ inductive Occurs : {n : Nat} → String → Term' n → Prop
 | app₁ {t₀ t₁ : Term' n} : Occurs v t₁ → Occurs v (app t₀ t₁)
 | lam {T} {t : Term' (succ n)} : Occurs v t → Occurs v (lam T t)
 
+open DecidableTotalOrder (pcompare)
+
+theorem abstr_inst' (v : Name) (k : Fin (succ n)) (k' : Fin m)
+        (t : Term' m) (hm : m = succ n) (hk : k.val = k'.val)
+        (hv : ¬ Occurs v t):
+  abstr v k (inst' k' (fvar v) hm t) = (hm ▸ t) := by
+induction t generalizing k n
+<;> subst hm
+<;> simp [inst', abstr, bump]
+next a =>
+  -- split
+  cases pcompare a.val k'.val
+  <;> simp [abstr]
+  next h₀ =>
+    have h₁ : ¬ k.val ≤ a.val := Nat.not_le_of_gt <| hk ▸ h₀
+    simp [if_neg h₁, Fin.widen]
+  next h₀ =>
+    apply Fin.val_inj
+    rw [h₀, hk]
+  next h₀ =>
+    have h₂ : 0 < a.val := Nat.lt_of_le_of_lt (Nat.zero_le _) h₀
+    have h₁ : k.val ≤ a.val - 1 := by
+      show _ ≤ a.val.pred
+      apply Nat.le_of_succ_le_succ
+      rw [Nat.succ_pred h₂, hk]; assumption
+    rw [if_pos h₁]; apply congrArg
+    apply Fin.val_inj; simp
+    apply Nat.le_antisymm
+    next =>
+      rw [Nat.succ_le_iff]; refl
+      apply Nat.lt_of_le_of_lt _ h₀
+      auto
+    next =>
+      rw [Preorder.indirect_le_r]; intro z
+      intro h; have h' := h
+      have h₃ : 0 < z :=
+        Nat.lt_of_le_of_lt (Nat.zero_le _) h'
+      rw [Nat.succ_le_iff h₃] at h
+      have h : succ a.val.pred ≤ _ := Nat.succ_le_succ h
+      simp [Nat.succ_pred,h₂,h₃] at h; assumption
+next =>
+  split
+  next h => subst h; auto [Occurs.fvar]
+  next => rfl
+next ih₀ ih₁ =>
+  rw [ih₀, ih₁] <;> auto
+next ih₀ ih₁ ih₂ =>
+  rw [ih₀, ih₁, ih₂] <;> auto
+next ih₀ ih₁ =>
+  rw [ih₀, ih₁] <;> auto
+next ih₀ =>
+  rw [ih₀]
+  . simp; assumption
+  . auto
+
+theorem abstr_inst (v : Name) (k : Fin (succ n)) (t : Term' (succ n))
+        (hv : ¬ Occurs v t) :
+  abstr v k (inst k (fvar v) t) = t := by
+simp [inst]; rw [abstr_inst'] <;> auto
+
+-- theorem abstr_inst₀ (v : Name) (k : Fin (succ n)) (t : Term' (succ n)) :
+--   abstr v k (inst k e t) = subst v _ t := sorry
+
+theorem inst_abstr (v v' : Name) (k : Fin (succ n)) (t : Term' n) :
+        -- (hv : ¬ Occurs v t) :
+  inst k e (abstr v k t) = subst v e t := by
+admit
+-- #check Lean.Name.
+
 def fresh' (n : Nat) : Term' k → Nat
 | fvar v =>
-  match String.toNat? <| v.drop 1 with
-  | none => n
-  | some n' => max n (n' + 1)
+  match v with
+  | Name.num p n' _ => max n (n' + 1)
+  | _ => n
 | bvar _ => n
 | plus t₀ t₁ =>
   let n := fresh' n t₀
@@ -78,8 +537,8 @@ def fresh' (n : Nat) : Term' k → Nat
   n
 | lam T t => fresh' n t
 
-def fresh (t : Term' n) : String :=
-"x" ++ toString (fresh' 0 t)
+def fresh (t : Term' n) : Name :=
+Name.mkNum `x (fresh' 0 t)
 
 theorem le_fresh' (t : Term' k)
   (h : m ≤ n) :
@@ -88,8 +547,10 @@ induction t generalizing n
 <;> simp [fresh', *]
 next =>
   split
-  next => auto
+  -- next =>
   next => auto [Nat.le_max_l]
+  next =>
+    auto
 next ihc ih₀ ih₁ => auto
   -- -- next => auto
   -- apply ih₁
@@ -99,7 +560,7 @@ next ihc ih₀ ih₁ => auto
 
 theorem not_Occurs_fresh (t : Term' n) :
   ¬ Occurs (fresh t) t := by
-suffices ∀ k n : Nat, Occurs ("x" ++ toString n) t → n < fresh' k t by
+suffices ∀ k n : Nat, Occurs (Name.mkNum `x n) t → n < fresh' k t by
   intro h; specialize this 0 _ h
   apply Nat.lt_irrefl _ this
 -- suffices ∀ k n : Nat, k ≤ n → Occurs ("x" ++ toString n) t → n < fresh' k t by
@@ -108,21 +569,14 @@ suffices ∀ k n : Nat, Occurs ("x" ++ toString n) t → n < fresh' k t by
 
 intros m k
 -- intros m k h₀
-generalize hv : "x" ++ toString k = v; intros h
+generalize hv : (`x).mkNum k = v; intros h
+-- have h' := h
 induction h generalizing m
 <;> simp [fresh']
+<;> try auto [le_fresh']
 next v' =>
-  have : String.toNat? (String.drop v' 1) = some k := by
-    rw [← hv]
-  simp [this]
+  simp [← hv, Name.mkNum]
   auto
-next ih =>
-  auto [le_fresh']
-next ih =>
-  apply ih _ hv
-next =>
-  auto [le_fresh']
-  -- split
 
 end Term'
 
@@ -134,15 +588,124 @@ export Term' (subst fvar plus ite app)
 open Term'
 
 -- opaque
-def lam (x : String) (T : Typ) (t : Term) : Term :=
-Term'.lam T (t.bump 0 |>.subst x <| bvar 0)
+def lam (x : Name) (T : Typ) (t : Term) : Term :=
+Term'.lam T (abstr x 0 t)
 
 open Term in
 inductive View : Term → Type
-| fvar {x} : View (fvar x)
-| plus {t₀ t₁} : View t₀ → View t₁ → View (plus t₀ t₁)
-| ite {c t₀ t₁} : View c → View t₀ → View t₁ → View (Term.ite c t₀ t₁)
-| app {t₀ t₁} : View t₀ → View t₁ → View (app t₀ t₁)
-| lam {x T t} : View t → View (lam x T t)
+| fvar {x} :      View (fvar x)
+| plus {t₀ t₁} :  View t₀ → View t₁ → View (plus t₀ t₁)
+| ite {c t₀ t₁} : View c  → View t₀ → View t₁ → View (Term.ite c t₀ t₁)
+| app {t₀ t₁} :   View t₀ → View t₁ → View (app t₀ t₁)
+| lam {x T t} :   View t  → View (lam x T t)
+
+-- def insts : (vs : List Name) → Term' vs.length → Term
+-- | [], t => t
+-- | v :: vs, t => insts vs <| inst 0 (fvar v) t
+-- #check Fin.cast
+def insts' (k : Nat) (vs : List (Term' k)) (h : n = vs.length + k) :
+  Term' n → Term' k
+| bvar i =>
+  if h' : i.val < k
+  then bvar <| i.cast h |>.cutl' h'
+  else vs.get <| i.cast h |>.cutr' h'
+  -- match Fin.split (i.cast h) with
+  -- | Sum.inl i => vs.get i
+  -- | Sum.inr i => bvar i
+| fvar x => fvar x
+| app t₀ t₁  => app (insts' k vs h t₀) (insts' k vs h t₁)
+| plus t₀ t₁ => plus (insts' k vs h t₀) (insts' k vs h t₁)
+| Term'.ite c t₀ t₁ =>
+  ite (insts' k vs h c) (insts' k vs h t₀) (insts' k vs h t₁)
+| Term'.lam T t =>
+Term'.lam T <|
+  insts' k.succ (bump 0 <$> vs)
+    (by simp [succ_add,h]) t
+
+open DecidableTotalOrder
+
+-- -- (by simp [h₀, Nat.succ_add])
+@[simp]
+theorem insts_cons
+        (vs : List (Term' k))
+        (t : Term' n)
+        (h₀ : n = List.length (t' :: vs) + k)
+        (h₁ : _ = _) :
+        -- (h₁ : n = List.length vs) :
+  insts' _ (t' :: vs) h₀ t =
+  inst' Fin.last t' rfl (insts' k.succ (bump 0 <$> vs) h₁ t) := by
+induction t
+ <;> simp [insts', Fin.split]
+next a =>
+  split; split
+  next h₀ h₁ =>
+    simp [inst']; split
+    next h₇ h₈ =>
+      clear h₈; simp [inst'] at *
+      rw [h₇] at h₀; cases Nat.lt_irrefl _ h₀
+    next =>
+      apply congrArg; apply Fin.val_inj
+      simp
+    next =>
+      skip
+      apply congrArg; apply Fin.val_inj
+      simp
+
+  -- next h => rw [h]
+  -- inst k _ (insts' (bump 0 <$> vs) _ t) := by
+--   -- insts' vs h₁ (inst' i t' (by simp [h₀, h₁]) t) := by
+-- induction t
+-- <;> simp [insts', inst']
+-- next j =>
+--   cases pcompare j.val i.val <;> simp [insts']
+--   next h₃ =>
+--     rw [h₂] at h₃; cases Nat.not_lt_zero _ h₃
+--   next h₃ =>
+--     rw [h₂] at h₃; cases j; subst h₃; rfl
+skip
+
+-- #exit
+
+def insts (vs : List (Term' m)) (t : Term' (vs.length + m)) : Term' m :=
+insts' _ vs rfl t
+
+-- #exit
+-- #check Nat.add
+def view' {vs} (hn : n = vs.length)
+  (hf : ∀ i, View (vs.get i)) :
+  (t : Term' n) → View (insts' 0 vs hn t)
+| bvar x =>
+  let x' : Fin (n + 0) := x
+  -- have h₀ : Fin.split (x.cast _ : Fin (vs.length + 0)) = Sum.inl (hn ▸ x : Fin vs.length) := by
+    -- simp [Fin.split]; rw [dif_pos]
+  have h₀ : x.val < List.length vs := hn ▸ x.isLt
+  suffices View (vs.get <| x.cast hn) by
+    simp [insts', dif_pos h₀]
+    exact this
+  hf _
+| fvar x => View.fvar
+| plus t₀ t₁ => View.plus (view' _ hf t₀) (view' _ hf t₁)
+| app t₀ t₁ => View.app (view' _ hf t₀) (view' _ hf t₁)
+| ite c t₀ t₁ => View.ite (view' _ hf c) (view' _ hf t₀) (view' _ hf t₁)
+| Term'.lam T t =>
+  let x := fresh t
+  show View (Term'.lam _ _) from
+  -- have h :=
+  by rw [← abstr_inst x 0 (insts' (succ 0) (bump 0 <$> vs) _ t)]
+     apply View.lam
+  -- by simp [insts']
+
+
+def view : (t : Term) → View t
+| fvar x => View.fvar
+| plus t₀ t₁ => View.plus (view t₀) (view t₁)
+| app t₀ t₁ => View.app (view t₀) (view t₁)
+| ite c t₀ t₁ => View.ite (view c) (view t₀) (view t₁)
+| Term'.lam T t =>
+  let x := fresh t
+  have : t = abstr x 0 (inst 0 (fvar x) t) :=
+    abstr_inst _ _ _ (Term'.not_Occurs_fresh _) |>.symm
+  -- View.lam <| view <| inst 0 (fvar x) t
+  _
 
 end Term
