lib/lib/Meta/TransportFacts.lean
@@ -1,0 +1,113 @@
+
+structure LockedType {T : Sort u} (T' : Sort u) (x : T) where
+  val : T'
+  type_eq : T = T'
+  val_eqv : HEq val x
+
+infix:50 " ~= " => HEq
+
+theorem Eq.toHEq {α} {x y : α} (h : x = y) : x ~= y :=
+by cases h; constructor
+
+theorem HEq.toEq {α} {x y : α} (h : x ~= y) : x = y :=
+by cases h; rfl
+
+namespace Transport
+
+class EqvTypes (T T' : Sort u) : Prop where
+  rfl : T = T'
+
+class EqvTerm {α α' : Sort u} [EqvTypes α α'] (x : α) (y : α') : Prop where
+  rfl : x ~= y
+
+  -- transport : T → T'
+  -- transport_eq x : HEq (transport x) x
+
+@[defaultInstance 100] /- low prio -/
+instance(priority := low) : EqvTypes T T where
+  rfl := rfl
+  -- transport := id
+  -- transport_eq x := HEq.rfl
+-- #check Lean.Meta.PrioritySet
+-- #fullname low
+-- #find prefix Priority
+-- #check Priority.low
+
+@[instance]
+def EqvTypes_arrow {α α' : Sort u} {β β' : Sort v}
+    [EqvTypes α α'] [EqvTypes β β'] :
+         EqvTypes (α → β) (α' → β') where
+  rfl := by rw [@EqvTypes.rfl α α', @EqvTypes.rfl β β']
+
+@[instance]
+def EqvTypes_forall {α α'} (h' : EqvTypes.{v} α α')
+  {β : α → Sort u}
+  {β' : α' → Sort u}
+  (h : ∀ (x : α) (y : α'), EqvTerm x y → EqvTypes (β x) (β' y)) :
+  EqvTypes (∀ x, β x) (∀ x, β' x) where
+    rfl := by
+      have := h'.rfl; subst this
+      have h₀ : ∀ x, β x = β' x :=
+        λ x => h x x ⟨ HEq.rfl ⟩ |>.rfl
+      have h₁ : β = β' := funext h₀
+      rw  [h₁]
+
+def EqvTerm_app {α α'} {β β'} (f : α → β) (g : α' → β') x y
+    (h₀ : EqvTypes α α')
+    (h₁ : EqvTypes β β')
+    (h₂ : EqvTerm f g)
+    (h₃ : EqvTerm x y) :
+  EqvTerm (f x) (g y) where
+    rfl := by
+      have := h₀.rfl; subst this
+      have := h₁.rfl; subst this
+      have := HEq.toEq h₂.rfl; subst this
+      have := HEq.toEq h₃.rfl; subst this
+      constructor
+
+def EqvTypes_of_EqvTerm {α α'} (h : EqvTerm α α') : EqvTypes α α' where
+  rfl := by
+    have := h.rfl; cases this
+    constructor
+
+macro "prove_transport" : tactic =>
+  `(tactic|
+    solve
+    | repeat
+        first
+        | intros _
+        | assumption
+        | apply EqvTypes_arrow
+        | apply EqvTypes_forall
+        | apply EqvTerm_app
+        | apply EqvTypes_of_EqvTerm
+        | exact inferInstance )
+
+instance (x : α) : EqvTerm x x where
+  rfl := HEq.rfl
+
+def transport α α' [EqvTypes α' α] (x : α) : α' :=
+cast EqvTypes.rfl.symm x
+
+def transport_eq α α' [EqvTypes α' α] (x : α) :
+  HEq (transport α α' x) x := by
+have h := @EqvTypes.rfl α' α _
+subst h
+constructor
+
+def mkLockedType (α) {α'} (x : α')
+    -- (h : EqvTypes α' α := by prove_transport) :
+    (h : EqvTypes α α' := by prove_transport) :
+    LockedType α x where
+  val := transport _ _ x
+  type_eq := EqvTypes.rfl.symm
+  val_eqv := transport_eq _ _ _
+
+def EqvTerm.ofEq {x y : α} (h : x = y) : EqvTerm x y where
+  rfl:= h.toHEq
+
+def EqvTerm.ofHEq {α β} [EqvTypes α β] {x : α} {y : β} (h : x ~= y) :
+    EqvTerm x y where
+  rfl:= h
+
+end Transport
