lib/lib/Meta/deBruijn_subtype.lean
@@ -1,0 +1,1336 @@
+
+import Lib.Data.Nat
+import Lib.Data.Ordering
+import Lib.Data.List.Basic
+import Lib.Meta.DeclGraph
+import Lib.Meta.Dump
+import Lib.Meta.Opaque
+import Lib.Meta.TransportFacts
+import Lib.Order.Basic
+
+macro_rules
+| `(tactic| decreasing_tactic) =>
+ `(tactic|
+   (simp [invImage, InvImage, Prod.lex, sizeOfWFRel, measure, Nat.lt_wfRel, WellFoundedRelation.rel]
+    repeat (first | apply Prod.Lex.right | apply Prod.Lex.left)
+    repeat (first | apply PSigma.Lex.right | apply PSigma.Lex.left)
+    simp [Nat.add_comm (n := 1), Nat.succ_add, Nat.mul_succ]
+    try apply Nat.lt_succ_of_le
+    repeat apply Nat.le_step
+    first
+    | repeat first | apply Nat.le_add_left | apply Nat.le_add_of_le_l
+    | assumption
+    all_goals apply Nat.le_refl ))
+-- #check @cast_eq
+-- theorem cast_eq {α} (h : α = α) (x) :
+  -- cast h x = x := rfl
+
+theorem cast_cast {α β} (h : α = β) (h' : β = α) (x) :
+  cast h (cast h' x) = x := by
+cases h; cases h'; rfl
+
+theorem cast_app {α α' β β'} (h : α' = α) (h' : β = β') (f : α → β) x :
+  cast h' (f (cast h x)) = (cast (by rw [h,h']) f : α' → β') x :=
+by substAll; simp [cast_eq]
+
+structure Equiv (α β : Sort u) where
+  to : α → β
+  inv : β → α
+  to_inv x : to (inv x) = x
+  inv_to x : inv (to x) = x
+
+attribute [simp] Equiv.to_inv Equiv.inv_to
+
+def Equiv.R (h : Equiv α β) x y :=
+h.to x = y ∧ x = h.inv y
+
+def Equiv.refl : Equiv α α where
+  to := id
+  inv := id
+  to_inv x := rfl
+  inv_to x := rfl
+
+def Equiv.symm (h₀ : Equiv α β) : Equiv β α where
+  to := h₀.inv
+  inv := h₀.to
+  inv_to := h₀.to_inv
+  to_inv := h₀.inv_to
+
+def Equiv.trans (h₀ : Equiv α β) (h₁ : Equiv β γ) : Equiv α γ where
+  to x  := h₁.to (h₀.to x)
+  inv x := h₀.inv (h₁.inv x)
+  to_inv x := by simp
+  inv_to x := by simp
+
+def Eq.toEquiv {α β : Type u} (h : α = β) : Equiv α β where
+  to  := cast h
+  inv := cast h.symm
+  to_inv := cast_cast _ _
+  inv_to := cast_cast _ _
+
+-- def Eq.toEquiv {α β : Type u} (h : Equiv α β) : α = β := _
+
+-- class EquivRel.{v,u} (T : Sort u) where
+--   R : T → T → Sort v
+--   refl x : R x x
+--   trans x y z : R x y → R y z → R x z
+--   -- to_eq x y : R x y → x = y
+
+class IsSetoid (α : Sort u) [HasEquiv α] where
+  refl (x : α) : x ≈ x
+  symm (x y : α) : x ≈ y → y ≈ x
+  trans (x y z : α) : x ≈ y → y ≈ z → x ≈ z
+
+instance : HasEquiv (Sort u) where
+  Equiv α β := Equiv α β
+
+instance : IsSetoid (Sort u) where
+  refl := @Equiv.refl
+  symm := @Equiv.symm
+  trans := @Equiv.trans
+-- #check Reflexive
+
+instance [HasEquiv.{v,u} α] [HasEquiv.{v',u'} β] : HasEquiv (α → β) where
+  Equiv f g := ∀ x y, HasEquiv.Equiv x y → HasEquiv.Equiv (f x) (g y)
+
+-- structure LockedType {T : Sort u} (T' : Sort u) [HasEquiv.{u,v} T] (x : T) where
+
+namespace Subtype
+
+theorem val_inj {p : α → Prop} {x y : Subtype p}
+        (h : x.val = y.val) :
+  x = y := by cases x; cases y; cases h; rfl
+
+end Subtype
+
+namespace Fin
+open Nat
+@[simp]
+protected def succ {n} : Fin n → Fin (succ n)
+| ⟨i,h⟩ => ⟨i.succ, Nat.succ_lt_succ h⟩
+
+def last : Fin (succ n) := ⟨n, Nat.lt_succ_self _⟩
+
+@[simp]
+def widen {n} : Fin n → Fin (succ n)
+| ⟨i,h⟩ => ⟨i, Nat.lt_succ_of_le <| Nat.le_of_lt h⟩
+
+def split {m n} : Fin (m + n) → Fin m ⊕ Fin n
+| ⟨i, h⟩ =>
+  if h' : i < m
+  then Sum.inl ⟨i, h'⟩
+  else
+    have : i - m < n :=
+      Nat.sub_lt_of_lt_add
+        (Nat.le_of_not_gt h') (Nat.add_comm n m ▸ h)
+    Sum.inr ⟨i - m, this⟩
+
+def cast (h : m = n) : Fin m → Fin n
+| ⟨i, h'⟩ => ⟨i, h ▸ h'⟩
+
+def cutl : (i : Fin (m + n)) → i.val < m → Fin m
+| ⟨i, h⟩, h' => ⟨i, h'⟩
+
+def cutr : (i : Fin (m + n)) → ¬ i.val < m → Fin n
+| ⟨i, h⟩, h' =>
+  have : i - m < n :=
+    Nat.sub_lt_of_lt_add
+      (Nat.le_of_not_gt h') (Nat.add_comm n m ▸ h)
+  ⟨i - m, this⟩
+
+def cutl' : (i : Fin (n + m)) → i.val < m → Fin m
+| ⟨i, h⟩, h' => ⟨i, h'⟩
+
+def cutr' : (i : Fin (n + m)) → ¬ i.val < m → Fin n
+| ⟨i, h⟩, h' =>
+  have : i - m < n :=
+    Nat.sub_lt_of_lt_add
+      (Nat.le_of_not_gt h') (Nat.add_comm n m ▸ h)
+  ⟨i - m, this⟩
+
+@[simp]
+theorem val_last :
+  (@Fin.last n).val = n := rfl
+
+@[simp]
+theorem val_cast (h : m = n) (i : Fin m) :
+  (i.cast h).val = i := rfl
+
+@[simp]
+theorem val_cutl (i : Fin (m + n)) h :
+  (i.cutl h).val = i.val := rfl
+
+@[simp]
+theorem val_cutr (i : Fin (m + n)) h :
+  (i.cutr h).val = i.val - m := rfl
+
+@[simp]
+theorem val_cutl' (i : Fin (m + n)) h :
+  (i.cutl' h).val = i.val := rfl
+
+@[simp]
+theorem val_cutr' (i : Fin (m + n)) h :
+  (i.cutr' h).val = i.val - n := rfl
+
+theorem val_inj {x y : Fin n} (h : x.val = y.val) : x = y :=
+by cases x; cases y; cases h; refl
+
+end Fin
+
+namespace List
+
+theorem get_eq_of_eq_0 {xs : List α} (i : Fin _)
+        (h : i.val = 0) :
+  (x :: xs).get i = x := by
+cases i; cases h
+simp [List.get]
+
+end List
+
+namespace Bool
+
+-- @[simp]
+-- theorem and_eq_true : (x && y) = true ↔ x = true ∧ y = true := by
+-- cases x <;> cases y <;> simp
+
+@[simp]
+theorem decide_eq_true [H : Decidable p] :
+  decide p = true ↔ p := by
+cases H <;> simp [decide] <;> assumption
+
+end Bool
+
+
+namespace Lean
+namespace Name
+
+-- @[simp]
+-- theorem beq_anonymous :
+--   (anonymous == anonymous) = true := rfl
+
+-- @[simp]
+-- theorem beq_num :
+--   (num p n h == num p' n' h') = true ↔
+--   (p == p') = true ∧ n = n' :=
+-- by simp [BEq.beq, Name.beq] <;> auto
+
+-- @[simp]
+-- theorem beq_str :
+--   (str p n h == str p' n' h') = true ↔
+--   (p == p') = true ∧ n = n' ∧ h = h' :=
+-- by simp [BEq.beq, Name.beq] <;> auto
+
+-- theorem beq_iff_eq {n n' : Name} :
+--   n == n' ↔ n = n' := by
+-- induction n generalizing n'
+-- <;> cases n'
+-- <;> next =>
+--   constructor <;> simp [*] <;> intro h
+--   <;> try (cases h) <;> try auto
+
+-- #exit
+instance : DecidableEq Name
+| n, n' =>
+  withPtrEqDecEq n n' λ () =>
+    match n, n' with
+    | anonymous, anonymous => isTrue rfl
+    | str p n h, str p' n' h' =>
+      have hh := (inferInstanceAs (Decidable (h = h')))
+      have hn := (inferInstanceAs (Decidable (n = n')))
+      have hp := instDecidableEqName p p'
+      have h := @instDecidableAnd _ _ hh (@instDecidableAnd _ _ hn hp)
+      @Decidable.congr _ _ h <| by
+        constructor <;> intro h
+        next =>
+          repeat
+            first
+            | rfl
+            | apply congr
+          all_goals auto
+        next => cases h; auto
+    | num p n h, num p' n' h' =>
+      have hh := (inferInstanceAs (Decidable (h = h')))
+      have hn := (inferInstanceAs (Decidable (n = n')))
+      have hp := instDecidableEqName p p'
+      have h := @instDecidableAnd _ _ hh (@instDecidableAnd _ _ hn hp)
+      @Decidable.congr _ _ h <| by
+        constructor <;> intro h
+        next =>
+          repeat
+            first
+            | rfl
+            | apply congr
+          all_goals auto
+        next => cases h; auto
+    | num _ _ _, str _ _ _ => isFalse λ h => by cases h
+    | num _ _ _, anonymous => isFalse λ h => by cases h
+    | str _ _ _, num _ _ _ => isFalse λ h => by cases h
+    | str _ _ _, anonymous => isFalse λ h => by cases h
+    | anonymous, num _ _ _ => isFalse λ h => by cases h
+    | anonymous, str _ _ _ => isFalse λ h => by cases h
+
+end Name
+end Lean
+
+
+inductive Typ : Type
+| nat | bool | arrow (t₀ t₁ : Typ)
+
+open Nat
+open Lean (Name)
+
+inductive NTerm' : Type
+| fvar : Name → NTerm'
+| plus (t₀ t₁ : NTerm') : NTerm'
+| ite (c t₀ t₁ : NTerm') : NTerm'
+| app (t₀ t₁ : NTerm') : NTerm'
+| lam : Name → Typ → NTerm' → NTerm'
+
+namespace NTerm'
+
+-- does not avoid capture. Ugh
+def subst (v : Name) (e : NTerm') : NTerm' → NTerm'
+| fvar n =>
+  if v == n then e else fvar n
+| plus t₀ t₁ =>
+  plus (subst v e t₀) (subst v e t₁)
+| app t₀ t₁ =>
+  app (subst v e t₀) (subst v e t₁)
+| ite c t₀ t₁ =>
+  ite (subst v e c) (subst v e t₀) (subst v e t₁)
+| lam x T t =>
+  if x == v then
+    lam x T t
+  else lam x T (subst v e t)
+
+inductive AlphaEqv : NTerm' → NTerm' → Prop
+| fvar : AlphaEqv (fvar v) (fvar v')
+| plus :
+  AlphaEqv ta₀ tb₀ → AlphaEqv ta₁ tb₁ →
+  AlphaEqv (plus ta₀ ta₁) (plus tb₀ tb₁)
+| app :
+  AlphaEqv ta₀ tb₀ → AlphaEqv ta₁ tb₁ →
+  AlphaEqv (app ta₀ ta₁) (app tb₀ tb₁)
+| ite :
+  AlphaEqv ca cb → AlphaEqv ta₀ tb₀ → AlphaEqv ta₁ tb₁ →
+  AlphaEqv (ite ca ta₀ ta₁) (ite cb tb₀ tb₁)
+| lam :
+  (∀ z, AlphaEqv (subst x (fvar z) ta) (subst y (fvar z) tb)) →
+  AlphaEqv (lam x T ta) (lam y T tb)
+
+end NTerm'
+
+inductive Term' : Type
+| bvar : Nat → Term'
+| fvar : Name → Term'
+| plus (t₀ t₁ : Term') : Term'
+| ite (c t₀ t₁ : Term') : Term'
+| app (t₀ t₁ : Term') : Term'
+| lam : Typ → Term' → Term'
+
+namespace Term'
+
+@[auto]
+inductive Bounded : Term' → Nat → Prop
+| bvar {v b} : v < b → Bounded (bvar v) b
+| fvar : Bounded (fvar n) b
+| plus : Bounded t₀ b → Bounded t₁ b → Bounded (plus t₀ t₁) b
+| ite : Bounded c b → Bounded t₀ b → Bounded t₁ b → Bounded (ite c t₀ t₁) b
+| app : Bounded t₀ b → Bounded t₁ b → Bounded (app t₀ t₁) b
+| lam : Bounded t (succ b) → Bounded (lam T t) b
+
+def bump (k : Nat) : Term' → Term'
+| bvar i =>
+  if k ≤ i then bvar i.succ else bvar i
+| fvar v => fvar v
+| plus t₀ t₁ => plus (bump k t₀) (bump k t₁)
+| Term'.ite c t₀ t₁ => ite (bump k c) (bump k t₀) (bump k t₁)
+| app t₀ t₁ => app (bump k t₀) (bump k t₁)
+| lam T t => lam T (bump k.succ t)
+
+def subst (v : Name) (e : Term') : Term' → Term'
+| bvar i => bvar i
+| fvar v' =>
+  if v = v' then e else fvar v'
+| plus t₀ t₁ => plus (subst v e t₀) (subst v e t₁)
+| Term'.ite c t₀ t₁ =>
+  ite (subst v e c) (subst v e t₀) (subst v e t₁)
+| app t₀ t₁ => app (subst v e t₀) (subst v e t₁)
+| lam T t' => lam T (subst v (bump 0 e) t')
+
+-- #print _sizeOf_inst
+-- #pred sizeOf
+
+-- inductive Subterm : ((n : Nat) × Term' n) → ((n : Nat) × Term' n) → Prop
+-- | plus₀ {n} {t₀ t₁ : Term' n} : Subterm ⟨n, t₀⟩ ⟨n, plus t₀ t₁⟩
+-- | plus₁ {n} {t₀ t₁ : Term' n} : Subterm ⟨n, t₁⟩ ⟨n, plus t₀ t₁⟩
+-- | app₀ {n} {t₀ t₁ : Term' n} : Subterm ⟨n, t₀⟩ ⟨n, app t₀ t₁⟩
+-- | app₁ {n} {t₀ t₁ : Term' n} : Subterm ⟨n, t₁⟩ ⟨n, app t₀ t₁⟩
+-- | itec {n} {c t₀ t₁ : Term' n} : Subterm ⟨n, c⟩ ⟨n, Term'.ite c t₀ t₁⟩
+-- | ite₀ {n} {c t₀ t₁ : Term' n} : Subterm ⟨n, t₀⟩ ⟨n, Term'.ite c t₀ t₁⟩
+-- | ite₁ {n} {c t₀ t₁ : Term' n} : Subterm ⟨n, t₁⟩ ⟨n, Term'.ite c t₀ t₁⟩
+-- | lam {n} {T} {t : Term' _} : Subterm ⟨_, t⟩ ⟨n, lam T t⟩
+
+@[simp]
+def height : Term' → Nat
+| bvar _ => 0
+| fvar _ => 0
+| plus t₀ t₁ => 1 + height t₀ + height t₁
+-- | plus t₀ t₁ => 1 + height t₀ + height t₁
+| app t₀ t₁ => 1 + height t₀ + height t₁
+-- | app t₀ t₁ => height t₀ + height t₁ + 1
+| Term'.ite c t₀ t₁ => 1 + height c + height t₀ + height t₁
+-- | Term'.ite c t₀ t₁ => height c + height t₀ + height t₁ + 1
+| lam T t => 1 + height t
+-- | lam T t => height t + 1
+
+-- namespace sizeOf
+
+-- variable {c t₀ t₁ : Term' n}
+-- variable (i : Fin 0)
+-- -- #eval sizeOf (@bvar 1 ⟨0, Nat.zero_lt_one⟩)
+-- #reduce sizeOf (bvar i)
+
+-- theorem _eq_1  : sizeOf (bvar i) = 1 :=
+-- show n.succ = _ from _
+
+-- end sizeOf
+
+
+-- set_option pp.explicit true in
+-- #check @sizeOf (Term' _) _
+-- #succ Term'
+-- #exit
+
+-- inductive A := | a
+
+-- def termWf : WellFoundedRelation ((n : Nat) × Term' n) where
+--   rel := Subterm
+--   wf := by
+--     constructor; intro a; cases a
+--     next n t =>
+--     induction t <;> constructor
+--     <;> intro a <;> cases a <;> intro h
+--     <;> cases h <;> assumption
+
+-- #check measure
+-- #check Nat.le_add_left
+attribute [scoped auto] Nat.le_add_left Nat.le_add_right Nat.succ_le_succ
+
+-- open Ordering in
+-- def inst {n} (k : Fin (succ n)) (e : Term' n) : Term' (succ n) → Term' n
+-- | bvar i =>
+--   match compare i.val k.val, rfl : (o : Ordering) → compare i.val k = o → _ with
+--   | eq, h => e
+--   | lt, h =>
+--     -- have h₀ : i.val < k.val := sorry
+--     have h₀ : i.val < k.val := by
+--       simp at h; assumption
+--     have h₁ : k.val ≤ n := Nat.le_of_succ_le_succ k.isLt
+--     bvar ⟨i.val, Nat.lt_of_lt_of_le h₀ h₁⟩
+--   | gt, h =>
+--     -- have : 1 ≤ i.val := sorry
+--     have : 1 ≤ i.val := by
+--       simp at h; trans _ </> assumption
+--       auto
+--     have : i.val - 1 < n := Nat.sub_lt_of_lt_add this i.isLt
+--     bvar ⟨i.val - 1,  this⟩
+-- | fvar v => fvar v
+-- | plus t₀ t₁ =>
+--        have : height t₀ < height (plus t₀ t₁) :=
+--          by simp [height];
+--             apply Nat.succ_le_succ
+--             apply Nat.le_add_right
+--          -- by simp [height]; auto
+--        have : height t₁ < height (plus t₀ t₁) :=
+--          by simp [height];
+--             apply Nat.succ_le_succ
+--             apply Nat.le_add_left
+--             -- apply Nat.le_add_of_le_r
+--          --    -- apply Nat.le_add_right
+--          -- by simp [height]; auto
+--        plus (inst k e t₀) (inst k e t₁)
+-- | Term'.ite c t₀ t₁ =>
+--        have : height c  < height (ite c t₀ t₁) :=
+--          by simp [height];
+--             apply Nat.succ_le_succ
+--             apply Nat.le_add_of_le_l
+--          --    -- apply Nat.le_add_right
+--             apply Nat.le_add_right
+--        have : height t₀ < height (ite c t₀ t₁) :=
+--          by simp [height];
+--             apply Nat.succ_le_succ
+--             apply Nat.le_add_of_le_l
+--          --    -- apply Nat.le_add_right
+--             apply Nat.le_add_left
+--          --    -- auto with 10
+--        have : height t₁ < height (ite c t₀ t₁) :=
+--          by simp [height];
+--             apply Nat.succ_le_succ
+--             -- apply Nat.le_add_of_le_l
+--             apply Nat.le_add_left
+--        ite (inst k e c) (inst k e t₀) (inst k e t₁)
+-- | app t₀ t₁ =>
+--        have : height t₀ < height (app t₀ t₁) :=
+--          by simp [height]
+--             apply Nat.succ_le_succ
+--             apply Nat.le_add_right
+--          -- by simp [height]; auto
+--        have : height t₁ < height (app t₀ t₁) :=
+--          by simp [height]
+--             apply Nat.succ_le_succ
+--             apply Nat.le_add_left
+--          --    -- auto with 17
+--        app (inst k e t₀) (inst k e t₁)
+-- | lam T t' =>
+--   -- have : height t' < height (lam T t') :=
+--          -- by simp [height]
+--             -- apply Nat.succ_le_succ
+--             -- apply Nat.le_add_left
+--             -- auto with 17
+--   lam T (inst k.succ (bump 0 e) t')
+-- -- termination_by' inst n k e t => Sigma.mk n t
+-- termination_by inst t => height t
+-- -- decreasing_by simp [InvImage]; try auto
+
+open POrdering DecidableTotalOrder in
+def inst' (k : Nat) (e : Term')  :
+  Term' → Term'
+| bvar i =>
+  -- have ⟨a, h⟩ : { a // compare i.val k.val = a } :=
+    -- ⟨ _,  rfl ⟩
+  match pcompare i k with
+  | isEQ h => e
+  | isLT h =>
+    -- have h₀ : i < k := by
+    --   simp at h; assumption
+    -- have h₁ : k ≤ m := Nat.le_of_succ_le_succ <| hn ▸ k.isLt
+    bvar i
+  | isGT h =>
+    -- have : 1 ≤ i.val := by
+    --   simp at h
+    --   trans k.val.succ <;> auto
+    -- have : i.val - 1 < m := Nat.sub_lt_of_lt_add this <| hn ▸ i.isLt
+    bvar <| i - 1
+| fvar v => fvar v
+| plus t₀ t₁ =>
+       -- have : height t₀ < height (plus t₀ t₁) :=
+       --   by simp [height];
+       --      apply Nat.succ_le_succ
+       --      apply Nat.le_add_right
+       --   -- by simp [height]; auto
+       -- have : height t₁ < height (plus t₀ t₁) :=
+       --   by simp [height];
+       --      apply Nat.succ_le_succ
+       --      apply Nat.le_add_left
+       --      -- apply Nat.le_add_of_le_r
+       --   --    -- apply Nat.le_add_right
+       --   -- by simp [height]; auto
+       plus (inst' k e t₀) (inst' k e t₁)
+| Term'.ite c t₀ t₁ =>
+       -- have : height c  < height (ite c t₀ t₁) :=
+       --   by simp [height];
+       --      apply Nat.succ_le_succ
+       --      apply Nat.le_add_of_le_l
+       --   --    -- apply Nat.le_add_right
+       --      apply Nat.le_add_right
+       -- have : height t₀ < height (ite c t₀ t₁) :=
+       --   by simp [height];
+       --      apply Nat.succ_le_succ
+       --      apply Nat.le_add_of_le_l
+       --   --    -- apply Nat.le_add_right
+       --      apply Nat.le_add_left
+       --   --    -- auto with 10
+       -- have : height t₁ < height (ite c t₀ t₁) :=
+       --   by simp [height];
+       --      apply Nat.succ_le_succ
+       --      -- apply Nat.le_add_of_le_l
+       --      apply Nat.le_add_left
+       ite (inst' k e c) (inst' k e t₀) (inst' k e t₁)
+| app t₀ t₁ =>
+       -- have : height t₀ < height (app t₀ t₁) :=
+       --   by simp [height]
+       --      apply Nat.succ_le_succ
+       --      apply Nat.le_add_right
+       --   -- by simp [height]; auto
+       -- have : height t₁ < height (app t₀ t₁) :=
+       --   by simp [height]
+       --      apply Nat.succ_le_succ
+       --      apply Nat.le_add_left
+       --   --    -- auto with 17
+       app (inst' k e t₀) (inst' k e t₁)
+| lam T t' =>
+  -- have : height t' < height (lam T t') :=
+         -- by simp [height]
+            -- apply Nat.succ_le_succ
+            -- apply Nat.le_add_left
+            -- auto with 17
+  lam T (inst' k.succ (bump 0 e) t')
+-- termination_by' inst n k e t => Sigma.mk n t
+-- termination_by inst t => height t
+-- decreasing_by simp [InvImage]; try auto
+
+-- def inst {n} (k : Fin (succ n)) (e : Term' n) : Term' (succ n) → Term' n :=
+-- inst' k e rfl
+
+def abstr (v : Name) (k : Nat) : Term' → Term'
+| bvar i =>
+  if k ≤ i then bvar i.succ
+  else bvar i
+| fvar v' =>
+  if v = v' then bvar k
+  else fvar v'
+| plus t₀ t₁ => plus (abstr v k t₀) (abstr v k t₁)
+| app t₀ t₁ => app (abstr v k t₀) (abstr v k t₁)
+| ite c t₀ t₁ => ite (abstr v k c) (abstr v k t₀) (abstr v k t₁)
+| lam T t => lam T (abstr v k.succ t)
+
+@[auto]
+inductive Occurs : Name → Term' → Prop
+| fvar : Occurs v (fvar v)
+| plus₀ {t₀ t₁ : Term'} : Occurs v t₀ → Occurs v (plus t₀ t₁)
+| plus₁ {t₀ t₁ : Term'} : Occurs v t₁ → Occurs v (plus t₀ t₁)
+| ite_c {c t₀ t₁ : Term'} : Occurs v c → Occurs v (ite c t₀ t₁)
+| ite₀ {c t₀ t₁ : Term'} : Occurs v t₀ → Occurs v (ite c t₀ t₁)
+| ite₁ {c t₀ t₁ : Term'} : Occurs v t₁ → Occurs v (ite c t₀ t₁)
+| app₀ {t₀ t₁ : Term'} : Occurs v t₀ → Occurs v (app t₀ t₁)
+| app₁ {t₀ t₁ : Term'} : Occurs v t₁ → Occurs v (app t₀ t₁)
+| lam {T} {t : Term'} : Occurs v t → Occurs v (lam T t)
+
+open DecidableTotalOrder (pcompare)
+
+theorem abstr_inst' (v : Name) (k : Nat) (t : Term')
+        (hv : ¬ Occurs v t):
+  abstr v k (inst' k (fvar v) t) = t := by
+induction t generalizing k
+-- <;> subst hm
+<;> simp [inst', abstr, bump]
+<;> try solve | simp [*]
+next a =>
+  -- split
+  cases pcompare a k
+  <;> simp [abstr, inst']
+  next h₀ =>
+    have h₁ : ¬ k ≤ a := Nat.not_le_of_gt h₀
+    simp [if_neg h₁]
+  next h₀ => exact h₀.symm
+  next h₀ =>
+    have h₂ : 0 < a := Nat.lt_of_le_of_lt (Nat.zero_le _) h₀
+    have h₆ : succ (pred a) = a :=
+      by rw [Nat.succ_pred h₂]
+    have h₅ : succ (a - 1) = a := h₆
+    have h₁ : k ≤ a - 1 := by
+      apply Nat.le_of_succ_le_succ
+      rw [h₅]; assumption
+    rw [if_pos h₁]; apply congrArg
+    apply Nat.le_antisymm
+    next =>
+      rw [Nat.succ_le_iff]; refl
+      apply Nat.lt_of_le_of_lt _ h₀
+      auto
+    next =>
+      rw [Preorder.indirect_le_r]; intro z
+      intro h; have h' := h
+      have h₃ : 0 < z :=
+        Nat.lt_of_le_of_lt (Nat.zero_le _) h'
+      rw [Nat.succ_le_iff h₃] at h
+      have h : succ a.pred ≤ _ := Nat.succ_le_succ h
+      simp [Nat.succ_pred,h₂,h₃] at h; assumption
+next =>
+  split
+  next h => subst h; auto [Occurs.fvar]
+  next => rfl
+next ih₀ ih₁ =>
+  rw [ih₀, ih₁] <;> auto
+next ih₀ ih₁ ih₂ =>
+  rw [ih₀, ih₁, ih₂] <;> auto
+next ih₀ ih₁ =>
+  rw [ih₀, ih₁] <;> auto
+next ih₀ =>
+  rw [ih₀]; auto
+
+theorem abstr_inst (v : Name) (k : Nat) (t : Term')
+        (hv : ¬ Occurs v t) :
+  abstr v k (inst' k (fvar v) t) = t := by
+simp [inst']; rw [abstr_inst'] <;> auto
+
+-- theorem abstr_inst₀ (v : Name) (k : Fin (succ n)) (t : Term' (succ n)) :
+--   abstr v k (inst k e t) = subst v _ t := sorry
+
+theorem inst_abstr (v v' : Name) (k : Nat) (t : Term') :
+        -- (hv : ¬ Occurs v t) :
+  inst' k e (abstr v k t) = subst v e t := by
+admit
+
+-- #check Lean.Name.
+
+def fresh' (n : Nat) : Term' → Nat
+| fvar v =>
+  match v with
+  | Name.num p n' _ => max n (n' + 1)
+  | _ => n
+| bvar _ => n
+| plus t₀ t₁ =>
+  let n := fresh' n t₀
+  let n := fresh' n t₁
+  n
+| ite c t₀ t₁ =>
+  let n := fresh' n c
+  let n := fresh' n t₀
+  let n := fresh' n t₁
+  n
+| app t₀ t₁ =>
+  let n := fresh' n t₀
+  let n := fresh' n t₁
+  n
+| lam T t => fresh' n t
+
+def fresh (t : Term') : Name :=
+Name.mkNum `x (fresh' 0 t)
+
+theorem le_fresh' (t : Term')
+  (h : m ≤ n) :
+  m ≤ fresh' n t := by
+induction t generalizing n
+<;> simp [fresh', *]
+next =>
+  split
+  -- next =>
+  next => auto [Nat.le_max_l]
+  next =>
+    auto
+next ihc ih₀ ih₁ => auto
+  -- -- next => auto
+  -- apply ih₁
+  -- apply ih₀
+  -- apply ihc
+
+
+theorem not_Occurs_fresh (t : Term') :
+  ¬ Occurs (fresh t) t := by
+suffices ∀ k n : Nat, Occurs (Name.mkNum `x n) t → n < fresh' k t by
+  intro h; specialize this 0 _ h
+  apply Nat.lt_irrefl _ this
+-- suffices ∀ k n : Nat, k ≤ n → Occurs ("x" ++ toString n) t → n < fresh' k t by
+  -- intro h; specialize this 0 _ (Nat.zero_le _) h
+  -- apply Nat.lt_irrefl _ this
+
+intros m k
+-- intros m k h₀
+generalize hv : (`x).mkNum k = v; intros h
+-- have h' := h
+induction h generalizing m
+<;> simp [fresh']
+<;> try auto [le_fresh']
+next v' =>
+  simp [← hv, Name.mkNum]
+  auto
+
+-- namespace Bounded
+
+-- @[auto]
+-- theorem Bounded_plus
+--         (h₀ : Bounded t₀ n)
+--         (h₁ : Bounded t₁ n) :
+--   Bounded (plus t₀ t₁) n := by
+
+@[auto]
+theorem Bounded_bump
+        (h : Bounded t n) :
+  Bounded (bump k t) (succ n) := by
+induction h generalizing k <;> simp [bump]
+<;> split* <;> auto
+
+@[auto]
+theorem Bounded_inst
+        (h₀ : Bounded x n)
+        (h₁ : Bounded t (succ n))
+        (h₂ : k ≤ n) :
+  Bounded (inst' k x t) n := by
+induction t generalizing x n k
+<;> simp [inst']
+<;> cases h₁
+<;> solve
+    | split*
+      <;> auto
+split <;>
+  repeat
+    first
+    | assumption
+    | constructor
+case bvar.bvar.h_2.a h₀ h₁ =>
+  apply Nat.lt_of_lt_of_le h₀ h₂
+case bvar.bvar.h_3.a a _ h₀ h₁ h₂ =>
+  apply Nat.le_of_succ_le_succ
+  have → : succ (a - 1) = a := by
+    show succ (pred a) = a
+    rw [Nat.succ_pred]
+    apply Nat.lt_of_le_of_lt (m := k) <;> auto
+  assumption
+
+@[auto]
+theorem Bounded_abstr
+        (h : Bounded t n)
+        (h' : k ≤ n) :
+  Bounded (abstr x k t) (succ n) := by
+induction t generalizing n k
+<;> simp [abstr]
+<;> cases h
+<;> solve
+    | split*
+      <;> auto
+
+end Term'
+  -- transport x := cast (by rw [@EqvTypes.rfl α α', @EqvTypes.rfl β β']) x
+  -- transport_eq x := by
+  --   have h₀ := @EqvTypes.rfl α α' _
+  --   have h₁ := @EqvTypes.rfl β β' _
+  --   substAll
+  --   constructor
+
+namespace Term.Impl
+open Transport
+
+-- def Term := { t // Term'.Bounded t 0 }
+opaque def Term := { t // Term'.Bounded t 0 }
+
+-- #pred HEq
+
+@[auto]
+instance : EqvTypes Term._def Term where
+  rfl := Term._unlock.symm
+  -- transport x := cast Term._unlock.symm x
+  -- transport_eq x := by
+  --   have h := Term._unlock
+
+
+-- export Term' (subst fvar plus ite app)
+open Term'
+
+-- -- #print Eq
+-- -- @[elab declaration]
+-- -- def elabDeclaration : Lean.Elab.Command.CommandElab := fun stx => do
+--   -- throwError "my elab"
+-- elab_rules : command
+-- | `($d:«def») => _
+
+-- elab_rules : command
+-- | `($d:declaration) => println!"my elab"
+-- elab (d:declaration) : command =>
+--   println!"my elab"
+
+-- opaque
+-- @[transport foo]
+def fvar (x : Name) : Term._def :=
+⟨ Term'.fvar x, by auto ⟩
+
+#exit
+
+constant fvar_locked : LockedType (Name → Term) (fvar) :=
+mkLockedType _ _
+
+def fvar' : Name → Term := fvar_locked.val
+
+theorem fvar'._unlock : fvar' ~= fvar := fvar_locked.val_eqv
+
+@[auto]
+instance : EqvTerm fvar fvar' where
+  rfl := fvar'._unlock.symm
+
+-- opaque
+def plus : Term._def → Term._def → Term._def
+| ⟨t₀,h₀⟩, ⟨t₁,h₁⟩ =>
+⟨ Term'.plus t₀ t₁, by auto ⟩
+
+constant plus_locked : LockedType (Term → Term → Term) plus :=
+mkLockedType _ _
+
+def plus' : Term → Term → Term := plus_locked.val
+
+theorem plus'._unlock : plus' ~= plus := plus_locked.val_eqv
+
+instance : EqvTerm plus plus' where
+  rfl := plus'._unlock.symm
+
+-- opaque
+def app : Term._def → Term._def → Term._def
+| ⟨t₀,h₀⟩, ⟨t₁,h₁⟩ =>
+⟨ Term'.app t₀ t₁, by auto ⟩
+
+constant app_locked : LockedType (Term → Term → Term) app :=
+mkLockedType _ _
+
+def app' : Term → Term → Term := app_locked.val
+
+theorem app'._unlock : app' ~= app := app_locked.val_eqv
+
+instance : EqvTerm app app' where
+  rfl := app'._unlock.symm
+
+-- opaque
+def ite : Term._def → Term._def → Term._def → Term._def
+| ⟨c,hc⟩, ⟨t₀,h₀⟩, ⟨t₁,h₁⟩ =>
+⟨ Term'.ite c t₀ t₁, by auto ⟩
+
+constant ite_locked : LockedType (Term → Term → Term → Term) ite :=
+mkLockedType _ _
+
+def ite' : Term → Term → Term → Term := ite_locked.val
+
+theorem ite'._unlock : ite' ~= ite := ite_locked.val_eqv
+
+instance : EqvTerm ite ite' where
+  rfl := ite'._unlock.symm
+
+-- opaque
+def lam (x : Name) (T : Typ) : Term._def → Term._def
+| ⟨t, ht⟩ =>
+⟨Term'.lam T (abstr x 0 t), by auto ⟩
+
+constant lam_locked : LockedType (Name → Typ → Term → Term) lam :=
+mkLockedType _ _
+
+def lam' : Name → Typ → Term → Term := lam_locked.val
+
+theorem lam'._unlock : lam' ~= lam := lam_locked.val_eqv
+
+-- #exit
+
+def inst (x : Name) (t : Term') (h : Bounded t 1) : Term._def :=
+⟨ Term'.inst' 0 (Term'.fvar x) t, by auto ⟩
+
+@[simp]
+theorem val_lam : (lam x T t).val = Term'.lam T (abstr x 0 t.val) := rfl
+
+@[simp]
+theorem val_inst : (inst x t h).val = inst' 0 (Term'.fvar x) t := rfl
+
+open Term in
+inductive View : Term._def → Type
+| fvar {x} :      View (fvar x)
+| plus {t₀ t₁} :  View t₀ → View t₁ → View (plus t₀ t₁)
+| ite {c t₀ t₁} : View c  → View t₀ → View t₁ → View (ite c t₀ t₁)
+| app {t₀ t₁} :   View t₀ → View t₁ → View (app t₀ t₁)
+| lam {x T t} :   View t  → View (lam x T t)
+
+-- -- def insts : (vs : List Name) → Term' vs.length → Term
+-- -- | [], t => t
+-- -- | v :: vs, t => insts vs <| inst 0 (fvar v) t
+-- -- #check Fin.cast
+-- def insts' (k : Nat) (vs : List (Term' k)) (h : n = vs.length + k) :
+--   Term' n → Term' k
+-- | bvar i =>
+--   if h' : i.val < k
+--   then bvar <| i.cast h |>.cutl' h'
+--   else vs.get <| i.cast h |>.cutr' h'
+--   -- match Fin.split (i.cast h) with
+--   -- | Sum.inl i => vs.get i
+--   -- | Sum.inr i => bvar i
+-- | fvar x => fvar x
+-- | app t₀ t₁  => app (insts' k vs h t₀) (insts' k vs h t₁)
+-- | plus t₀ t₁ => plus (insts' k vs h t₀) (insts' k vs h t₁)
+-- | Term'.ite c t₀ t₁ =>
+--   ite (insts' k vs h c) (insts' k vs h t₀) (insts' k vs h t₁)
+-- | Term'.lam T t =>
+-- Term'.lam T <|
+--   insts' k.succ (bump 0 <$> vs)
+--     (by simp [succ_add,h]) t
+
+open DecidableTotalOrder
+
+-- -- -- (by simp [h₀, Nat.succ_add])
+-- @[simp]
+-- theorem insts_cons
+--         (vs : List (Term' k))
+--         (t : Term' n)
+--         (h₀ : n = List.length (t' :: vs) + k)
+--         (h₁ : _ = _) :
+--         -- (h₁ : n = List.length vs) :
+--   insts' _ (t' :: vs) h₀ t =
+--   inst' Fin.last t' rfl (insts' k.succ (bump 0 <$> vs) h₁ t) := by
+-- induction t
+--  <;> simp [insts', Fin.split]
+-- next a =>
+--   split; split
+--   next h₀ h₁ =>
+--     simp [inst']; split
+--     next h₇ h₈ =>
+--       clear h₈; simp [inst'] at *
+--       rw [h₇] at h₀; cases Nat.lt_irrefl _ h₀
+--     next =>
+--       apply congrArg; apply Fin.val_inj
+--       simp
+--     next =>
+--       skip
+--       apply congrArg; apply Fin.val_inj
+--       simp
+
+--   -- next h => rw [h]
+--   -- inst k _ (insts' (bump 0 <$> vs) _ t) := by
+-- --   -- insts' vs h₁ (inst' i t' (by simp [h₀, h₁]) t) := by
+-- -- induction t
+-- -- <;> simp [insts', inst']
+-- -- next j =>
+-- --   cases pcompare j.val i.val <;> simp [insts']
+-- --   next h₃ =>
+-- --     rw [h₂] at h₃; cases Nat.not_lt_zero _ h₃
+-- --   next h₃ =>
+-- --     rw [h₂] at h₃; cases j; subst h₃; rfl
+-- skip
+
+-- -- #exit
+
+-- def insts (vs : List (Term' m)) (t : Term' (vs.length + m)) : Term' m :=
+-- insts' _ vs rfl t
+
+-- -- @[simp]
+-- theorem dec_1 p q : p < 1 + p + q := sorry
+-- theorem dec_2 p q : q < 1 + p + q := sorry
+
+@[simp]
+theorem height_inst' k x t :
+  height (inst' k (Term'.fvar x) t) = height t := by
+induction t generalizing k
+<;> simp [inst', *, bump]
+split <;> rfl
+
+-- @[simp]
+-- theorem dec_3 p q : p < q + p ↔ 0 < q := sorry
+attribute [scoped simp] inst' in
+-- #exit
+-- #check Nat.add
+def view' :
+  (t : Term') → (h : Bounded t 0) → View ⟨t,h⟩
+-- | bvar x, Bounded =>
+  -- let x' : Fin (n + 0) := x
+  -- have h₀ : Fin.split (x.cast _ : Fin (vs.length + 0)) = Sum.inl (hn ▸ x : Fin vs.length) := by
+    -- simp [Fin.split]; rw [dif_pos]
+  -- have h₀ : x.val < List.length vs := hn ▸ x.isLt
+  -- suffices View (vs.get <| x.cast hn) by
+  --   simp [insts', dif_pos h₀]
+  --   exact this
+  -- hf _
+
+| Term'.bvar x, h => False.elim <| by
+  cases h with | bvar h => cases (Nat.not_lt_zero _ h)
+| Term'.fvar x, h => View.fvar
+| Term'.plus t₀ t₁, h =>
+  have : height t₀ < 1 + height t₀ + height t₁ := sorry
+  have : height t₁ < 1 + height t₀ + height t₁ := sorry
+  View.plus (view' t₀ (by cases h; auto)) (view' t₁ (by cases h; auto))
+| Term'.app t₀ t₁, h =>
+  have : height t₀ < 1 + height t₀ + height t₁ := sorry
+  have : height t₁ < 1 + height t₀ + height t₁ := sorry
+  View.app (view' t₀ (by cases h; auto)) (view' t₁ (by cases h; auto))
+| Term'.ite c t₀ t₁, h =>
+  have : height c < 1 + height c + height t₀ + height t₁ := sorry
+  have : height t₀ < 1 + height c + height t₀ + height t₁ := sorry
+  have : height t₁ < 1 + height c + height t₀ + height t₁ := sorry
+  View.ite (view' c (by cases h; auto))
+    (view' t₀ (by cases h; auto))
+    (view' t₁ (by cases h; auto))
+| Term'.lam T t, h =>
+  let x := fresh t
+  -- cases h
+  have h₂ : Bounded t 1 := sorry
+  -- have h' : Bounded (Term'.lam T (abstr x 0 (inst' 0 (Term'.fvar x) t))) 0 := sorry
+  have : height t < 1 + height t := sorry
+  suffices View (lam x T (inst x t h₂)) by
+    -- unfold lam at this
+    have h' := not_Occurs_fresh t
+    apply cast _ this; apply congrArg
+    apply Subtype.val_inj
+    simp [abstr_inst', h']
+    -- h'; simp only [lam, inst]
+    -- simp [abstr_inst]
+    -- revert h'
+    -- apply not_Occurs_fresh
+  View.lam (view' (inst' _ _ t) _)
+  -- let x := fresh t
+  -- show View (Term'.lam _ _) from
+  -- -- have h :=
+  -- by rw [← abstr_inst x 0 (insts' (succ 0) (bump 0 <$> vs) _ t)]
+  --    apply View.lam
+  -- -- by simp [insts']
+termination_by view' t _ => height t
+
+def view :
+  (t : Term._def) → View t
+| ⟨t,ht⟩ => view' t ht
+
+section rec
+variable {motive : Term._def → Sort u}
+variable (Hvar : (v : Name) → motive (fvar v))
+variable (Happ : (t₀ t₁ : Term._def) → motive t₀ → motive t₁ → motive (app t₀ t₁))
+variable (Hplus : (t₀ t₁ : Term._def) → motive t₀ → motive t₁ → motive (plus t₀ t₁))
+variable (Hite : (c t₀ t₁ : Term._def) →
+         motive c → motive t₀ → motive t₁ →
+         motive (ite c t₀ t₁))
+variable (Hlam : ∀ x T,
+         (t : Term._def) →
+         motive t →
+         motive (lam x T t))
+
+def Hvar' : (v : Name) → motive (fvar v) := sorry
+
+elab "trace" : tactic => do
+  let g ← Lean.Elab.Tactic.getMainGoal
+  print_vars![Lean.asGoal g]
+
+-- macro "haveI " " : " p:term ":=" proof:term : term =>
+  -- `
+-- #print auto_db
+-- #check instEqvTypesForAllForAll
+-- set_option pp.explicit true in
+-- #check @Hvar'.{u}
+-- #check mkLockedType
+-- #check @instEqvTypesForAllForAll
+-- set_option trace.auto.lemmas true
+
+def new : LockedType
+  ({motive : Term → Sort u} → ((v : Name) → motive (fvar' v)))
+  (@Hvar'.{u}) :=
+-- have : EqvTypes (Term._def → Sort u) (Term → Sort u) :=
+--   inferInstance
+-- have : ∀ (x : Term._def → Sort u) (y : Term → Sort u),
+--      EqvTerm x y → EqvTypes
+--        (((v : Name) → x (fvar v)))
+--        ((v : Name) → y (fvar' v)) :=
+--      λ x y Hxy =>
+--        have : ∀ (n : Name) (n' : Name), EqvTerm n n' →
+--             EqvTypes (x (fvar n)) (y (fvar' n')) := sorry
+--        @instEqvTypesForAllForAll Name Name _ _ _
+--          -- (λ n => x (fvar n))
+--          -- (λ n => y (fvar' n))
+--          this
+-- have : EqvTypes
+--   ({motive : Term._def → Sort u} → ((v : Name) → motive (fvar v)))
+--   ({motive : Term → Sort u} → ((v : Name) → motive (fvar' v))) := by
+--   -- @instEqvTypesForAllForAll _ _ _ _ _ this
+--   -- eauto
+--   eauto_step
+--   focus
+--     eauto [bar_foo] with 15
+
+    -- eauto_step
+    -- admit
+    -- eauto_step
+  -- apply d
+  -- auto_step
+  -- auto_step
+  -- apply d
+  -- eauto_step
+  -- eauto_step
+  -- eauto_step
+  -- -- auto_step
+mkLockedType _
+  (by
+  prove_transport
+  )
+  _
+
+#exit
+
+def rec' : (t : Term._def) → View t → motive t
+| _, View.fvar => Hvar _
+| _, View.plus t₀ t₁ => Hplus _ _ (rec' _ t₀) (rec' _ t₁)
+| _, View.app t₀ t₁ => Happ _ _ (rec' _ t₀) (rec' _ t₁)
+| _, View.ite c t₀ t₁ => Hite _ _ _ (rec' _ c) (rec' _ t₀) (rec' _ t₁)
+| _, View.lam t => Hlam _ _ _ (rec' _ t)
+
+def rec (t : Term._def) : motive t :=
+rec' Hvar Happ Hplus Hite Hlam t (view t)
+
+
+-- have v := view t
+-- let motive' t (v : View t) := motive t
+-- show motive' t v
+-- skip
+-- refine View.rec _ _ _ _ _ v
+
+-- induction v <;>
+-- first
+-- | auto
+-- | try apply_assumption <;> assumption
+
+
+end rec
+
+end Term.Impl
+
+opaque def Term := Term.Impl.Term
+-- constant Term_def : LockedType Term.Impl.Term :=
+-- { val := Term.Impl.Term
+--   val_eqv := Equiv.refl }
+
+-- def Term._eqv : Term ≈ Term.Impl.Term :=
+-- by rw [Term._unlock]; apply Equiv.refl
+
+-- #exit
+
+namespace Term
+
+opaque def fvar (v : Name) : Term :=
+-- suffices Name → Term.Impl.Term
+  -- by rw [Term._unlock]; exact this
+cast Term._unlock.symm (Term.Impl.fvar v)
+
+opaque def app (t₀ t₁ : Term) : Term :=
+-- suffices Term.Impl.Term → Term.Impl.Term → Term.Impl.Term
+--   by rw [Term._unlock]; exact this
+-- Term.Impl.app
+cast Term._unlock.symm
+  (Impl.app (cast Term._unlock t₀) (cast Term._unlock t₁))
+
+opaque def ite (c t₀ t₁ : Term) : Term :=
+-- suffices Term.Impl.Term → Term.Impl.Term → Term.Impl.Term
+--   by rw [Term._unlock]; exact this
+-- Term.Impl.app
+cast Term._unlock.symm
+  (Impl.ite
+    (cast Term._unlock c)
+    (cast Term._unlock t₀) (cast Term._unlock t₁))
+
+--  : Term → Term → Term → Term :=
+-- suffices Term.Impl.Term → Term.Impl.Term → Term.Impl.Term → Term.Impl.Term
+--   by rw [Term._unlock]; exact this
+-- Term.Impl.ite
+
+opaque def plus (t₀ t₁ : Term) : Term :=
+cast Term._unlock.symm
+  (Impl.plus (cast Term._unlock t₀) (cast Term._unlock t₁))
+
+-- suffices Term.Impl.Term → Term.Impl.Term → Term.Impl.Term
+--   by rw [Term._unlock]; exact this
+-- Term.Impl.plus
+
+opaque def lam (n : Name) (T : Typ) (t : Term) : Term :=
+cast Term._unlock.symm
+  (Impl.lam n T (cast Term._unlock t))
+
+--  : Name → Typ → Term → Term :=
+-- suffices Name → Typ → Term.Impl.Term → Term.Impl.Term
+--   by rw [Term._unlock]; exact this
+-- Term.Impl.lam
+
+inductive Eqv : Term → Impl.Term → Type
+| fvar : Eqv (Term.fvar x) (Impl.fvar x)
+| plus : Eqv ta₀ tb₀ → Eqv ta₁ tb₁ →
+  Eqv (Term.plus ta₀ ta₁) (Impl.plus tb₀ tb₁)
+| app : Eqv ta₀ tb₀ → Eqv ta₁ tb₁ →
+  Eqv (Term.app ta₀ ta₁) (Impl.plus tb₀ tb₁)
+| ite : Eqv ca cb → Eqv ta₀ tb₀ → Eqv ta₁ tb₁ →
+  Eqv (Term.ite ca ta₀ ta₁) (Impl.ite cb tb₀ tb₁)
+| lam : Eqv ta tb →
+  Eqv (Term.lam x T ta) (Impl.lam x T tb)
+
+
+-- inductive View : Term → Type
+-- | fvar {x} :      View (fvar x)
+-- | plus {t₀ t₁} :  View t₀ → View t₁ → View (plus t₀ t₁)
+-- | ite {c t₀ t₁} : View c  → View t₀ → View t₁ → View (ite c t₀ t₁)
+-- | app {t₀ t₁} :   View t₀ → View t₁ → View (app t₀ t₁)
+-- | lam {x T t} :   View t  → View (lam x T t)
+
+-- noncomputable def View.equiv.to : {t : Term} → {t' : Impl.Term} → Eqv t t' →
+--    (View t) → (Impl.View t')
+-- | _, _, Eqv.fvar, View.fvar => Impl.View.fvar
+-- | _, _, Eqv.plus h₀ h₁, _ => _
+-- | _, _, Eqv.app h₀ h₁, _ => _
+-- | _, _, Eqv.ite hc h₀ h₁, _ => _
+-- | _, _, Eqv.lam h₁, _ => _
+
+-- def View.equiv {t t'} : Eqv t t' →
+--   Equiv (View t) (Impl.View t') := by
+-- intro h
+-- -- cases t' with | mk t' ht' =>
+-- -- have v := Impl.view t'
+-- induction h with
+-- | fvar =>
+--   skip
+
+
+
+-- def view t : View t := by
+-- obtain ⟨t', ht⟩ : { t' : Impl.Term // t = cast Term._unlock.symm t' }
+--   from ⟨_, cast_cast Term._unlock.symm Term._unlock t |>.symm  ⟩
+-- have h := Impl.view t'
+-- cases h
+-- <;> rw [ht]
+
+-- opaque def view :
+
+theorem cast_app' {α α' β β'} (h : α = α') (h' : β = β') (f : α → β) x :
+  cast h' (f x) = (cast (by rw [h,h']) f : α' → β') (cast h x) :=
+by rw [← cast_app h.symm h', cast_cast]
+
+theorem cast_app'' {α β β'} (h' : β = β') (f : α → β) x :
+  cast h' (f x) = (cast (by rw [h']) f : α → β') x :=
+cast_app' rfl _ f x
+
+-- #print fvar._def
+
+section rec
+variable {motive : Term → Sort u}
+variable (Hvar : (v : Name) → motive (fvar v))
+variable (Happ : (t₀ t₁ : Term) → motive t₀ → motive t₁ → motive (app t₀ t₁))
+variable (Hplus : (t₀ t₁ : Term) → motive t₀ → motive t₁ → motive (plus t₀ t₁))
+variable (Hite : (c t₀ t₁ : Term) →
+         motive c → motive t₀ → motive t₁ →
+         motive (ite c t₀ t₁))
+variable (Hlam : ∀ x T,
+         (t : Term) →
+         motive t →
+         motive (lam x T t))
+
+-- #eval Lean.Meta.getUnfoldEqnFor? ``fvar._def
+-- #check app._unlock
+
+opaque def rec (t : Term) : motive t := by
+let motive' (t' : Impl.Term) := motive (cast Term._unlock.symm t')
+rw [← cast_cast Term._unlock.symm Term._unlock t]
+revert Hvar Happ Hplus Hite Hlam
+rw [fvar._unlock, app._unlock, plus._unlock, ite._unlock, lam._unlock]
+simp [fvar._def, app._def, plus._def, ite._def, lam._def]
+intros Hvar Happ Hplus Hite Hlam
+apply Impl.rec (motive := motive') <;> intros
+<;> simp
+next => apply Hvar
+next h₀ h₁ =>
+  specialize Happ _ _ h₀ h₁
+  simp only [cast_cast] at Happ
+  apply Happ
+next h₀ h₁ =>
+  specialize Hplus _ _ h₀ h₁
+  simp only [cast_cast] at Hplus
+  apply Hplus
+next hc h₀ h₁ =>
+  specialize Hite _ _ _ hc h₀ h₁
+  simp only [cast_cast] at Hite
+  apply Hite
+next h₀ =>
+  specialize Hlam _ _ _ h₀
+  simp only [cast_cast] at Hlam
+  apply Hlam
+
+-- #exit
+-- next =>
+--   simp; rw [cast_app'']
+--   generalize hk : cast _ _ = k
+--   have ← : fvar = k := by rw [← hk, fvar._unlock]; rfl
+--   auto
+-- next =>
+--   simp; rw [cast_app' Term._unlock]
+--   -- generalize hk : cast _ _ = k
+--   -- have ← : fvar = k := by rw [← hk, fvar._unlock]; rfl
+--   -- auto
+
+-- -- refine (cast )
+
+
+-- -- rw [Term._unlock] at t
+
+
+end rec
+
+end Term
