lib/lib/Meta/test2.lean
@@ -1,0 +1,37 @@
+
+import Lib.Meta.Opaque
+
+namespace Bar
+namespace Foo
+
+-- set_option trace.opaque.decls true
+opaque def Term := Unit
+end Foo
+
+#check Foo.Term._locked
+-- #check _impl.Term
+#check Foo.Term._impl.Term
+
+namespace Foo
+-- #check Term.instEqvTerm
+-- local notation "Term" => Term._def
+-- section A
+opaque namespace Term
+
+set_option trace.opaque true
+open Lean
+-- @[transport foo]
+def fvar (x : Name) : Term :=
+()
+
+def rec {motive : Term → Sort u} (f : ∀ n, motive (fvar n)) : ∀ t, motive t :=
+sorry
+
+-- #check foo
+#print Foo.Term.fvar._locked
+#check Foo.Term.fvar
+-- end Term._impl
+
+end Term
+#print Foo.Term._impl.fvar
+end Foo
